Add support for more general monad type in the translator. Split the functions and the proofs between files.
Still bugs to fix.

candle/standard/cf_kernel/ml_monadProgScript.sml
@@ -1,8 +1,23 @@
 open preamble ml_translatorTheory ml_translatorLib ml_pmatchTheory patternMatchesTheory
-open astTheory libTheory bigStepTheory semanticPrimitivesTheory holKernelTheory
+open astTheory libTheory bigStepTheory semanticPrimitivesTheory
 open terminationTheory ml_progLib ml_progTheory
 open set_sepTheory cfTheory cfStoreTheory cfTacticsLib Satisfy
 open cfHeapsBaseTheory basisFunctionsLib AC_Sort
+
+open ml_monadBaseTheory
+
+val _ = new_theory "ml_monadProg";
+
+val _ = temp_overload_on ("monad_bind", ``st_ex_bind``);
+val _ = temp_overload_on ("monad_unitbind", ``\x y. st_ex_bind x (\z. y)``);
+val _ = temp_overload_on ("monad_ignore_bind", ``\x y. st_ex_bind x (\z. y)``);
+val _ = temp_overload_on ("ex_bind", ``st_ex_bind``);
+val _ = temp_overload_on ("ex_return", ``st_ex_return``);
+
+val _ = temp_overload_on ("CONTAINER", ``ml_translator$CONTAINER``);
+
+
+val HCOND_EXTRACT = cfLetAutoTheory.HCOND_EXTRACT;
 
 (*********** Comes from cfLetAutoLib.sml ***********************************************)	 
 (* [dest_pure_fact]
@@ -14,24 +29,55 @@ fun dest_pure_fact p =
     (if same_const set_sep_cond_tm (#1 dp) then (#2 dp)
     else raise (ERR "dest_pure_fact" "Not a pure fact"))
   | _ => raise (ERR "dest_pure_fact" "Not a pure fact");
-
 (***************************************************************************************)
-		       
-val _ = new_theory "ml_monadProg";
+
+fun PURE_FACTS_FIRST_CONV H =
+  let
+      val preds = list_dest dest_star H
+      val (pfl, hpl) = List.partition (can dest_pure_fact) preds
+      val ordered_preds = pfl @ hpl
+  in
+      if List.null ordered_preds then REFL H
+      else
+	  let val H' = List.foldl (fn (x, y) => mk_star(y, x)) (List.hd ordered_preds)
+				  (List.tl ordered_preds)
+          (* For some strange reason, AC_CONV doesn't work *)
+          val H_to_norm = STAR_AC_CONV H
+	  val norm_to_H' = (SYM(STAR_AC_CONV H') handle UNCHANGED => REFL H')
+	  in TRANS H_to_norm norm_to_H'
+	  end
+  end;
+
+val EXTRACT_PURE_FACTS_CONV =
+  (RATOR_CONV PURE_FACTS_FIRST_CONV)
+  THENC (SIMP_CONV pure_ss [GSYM STAR_ASSOC])
+  THENC (SIMP_CONV pure_ss [HCOND_EXTRACT])
+  THENC (SIMP_CONV pure_ss [STAR_ASSOC]);
+
+(* TODO: use EXTRACT_PURE_FACT_CONV to rewrite EXTRACT_PURE_FACTS_TAC *)
+fun EXTRACT_PURE_FACTS_TAC (g as (asl, w)) =
+  let
+      fun is_hprop a = ((dest_comb a |> fst |> type_of) = ``:hprop`` handle HOL_ERR _ => false)
+      val hpreds = List.filter is_hprop asl
+      val hpreds' = List.map (fst o dest_comb) hpreds
+      val hpreds_eqs = List.map (PURE_FACTS_FIRST_CONV) hpreds'
+  in
+      ((fs hpreds_eqs) >> fs[GSYM STAR_ASSOC] >> fs[HCOND_EXTRACT] >> fs[STAR_ASSOC]) g
+  end;
+(***********************************************************************************************)
 
 val _ = temp_type_abbrev("state",``:'ffi semanticPrimitives$state``);
 
-fun auto_prove proof_name (goal,tac) = let
+(* fun auto_prove proof_name (goal,tac) = let
   val (rest,validation) = tac ([],goal) handle Empty => fail()
   in if length rest = 0 then validation [] else let
   in failwith("auto_prove failed for " ^ proof_name) end end
 
 fun D th = let
   val th = th |> DISCH_ALL |> PURE_REWRITE_RULE [AND_IMP_INTRO]
-  in if is_imp (concl th) then th else DISCH T th end
+  in if is_imp (concl th) then th else DISCH T th end *)
 
 (* a few basics *)
-
 val with_same_refs = Q.store_thm("with_same_refs",
   `(s with refs := s.refs) = s`,
   simp[state_component_equality])
@@ -40,294 +86,9 @@ val with_same_ffi = Q.store_thm("with_same_ffi",
   `(s with ffi := s.ffi) = s`,
   simp[state_component_equality]);
 
-
-val _ = (use_full_type_names := false);
-
-val _ = register_type ``:cpn``;
-val _ = register_type ``:'a # 'b``;
-val _ = register_type ``:'a list``;
-val _ = register_type ``:'a option``;
-
-val _ = ml_prog_update (open_module "Kernel");
-
-(* construct type refinement invariants *)
-
-val _ = register_type ``:type``;
-
-val MEM_type_size = Q.prove(
-  `!ts t. MEM t ts ==> type_size t < type1_size ts`,
-  Induct \\ FULL_SIMP_TAC (srw_ss()) [] \\ REPEAT STRIP_TAC \\ RES_TAC
-  \\ EVAL_TAC \\ FULL_SIMP_TAC std_ss [] \\ DECIDE_TAC);
-
-val type_ind = Q.store_thm("type_ind",
-  `(!s ts. (!t. MEM t ts ==> P t) ==> P (Tyapp s ts)) /\
-    (!v. P (Tyvar v)) ==> !x. P x`,
-  REPEAT STRIP_TAC \\ completeInduct_on `type_size x`
-  \\ REPEAT STRIP_TAC \\ FULL_SIMP_TAC std_ss [PULL_FORALL]
-  \\ Cases_on `x` \\ FULL_SIMP_TAC std_ss []
-  \\ Q.PAT_X_ASSUM `!x1 x2. bb` MATCH_MP_TAC
-  \\ REPEAT STRIP_TAC \\ Q.PAT_X_ASSUM `!x.bbb` MATCH_MP_TAC
-  \\ EVAL_TAC \\ IMP_RES_TAC MEM_type_size \\ DECIDE_TAC);
-
-val TYPE_TYPE_def = fetch "-" "TYPE_TYPE_def"
-
-val LIST_TYPE_NO_CLOSURES = Q.prove(
-  `!xs v.
-      (!x v. MEM x xs /\ p x v ==> no_closures v) /\
-      LIST_TYPE p xs v ==> no_closures v`,
-  Induct \\ FULL_SIMP_TAC std_ss [LIST_TYPE_def]
-  \\ REPEAT STRIP_TAC \\ FULL_SIMP_TAC std_ss [no_closures_def,EVERY_DEF,MEM]
-  \\ METIS_TAC []);
-
-val LIST_TYPE_11 = Q.prove(
-  `!P ts v1 us v2.
-      (!x1.
-       MEM x1 ts ==>
-        !v1 x2 v2.
-          P x1 v1 /\ P x2 v2 ==>
-          types_match v1 v2 /\ ((v1 = v2) <=> (x1 = x2))) /\
-    LIST_TYPE P ts v1 /\ LIST_TYPE P us v2 ==>
-    types_match v1 v2 /\ ((v1 = v2) = (ts = us))`,
-  STRIP_TAC \\ Induct \\ Cases_on `us` \\ FULL_SIMP_TAC (srw_ss()) []
-  \\ SIMP_TAC (srw_ss()) [LIST_TYPE_def,types_match_def,ctor_same_type_def]
-  \\ FULL_SIMP_TAC (srw_ss()) [PULL_EXISTS,types_match_def,ctor_same_type_def]
-  \\ METIS_TAC []);
-
-val CHAR_IMP_no_closures = Q.prove(
-  `CHAR x v ==> no_closures v`,
-  SIMP_TAC std_ss [CHAR_def,no_closures_def]);
-
-val STRING_IMP_no_closures = Q.prove(
-  `STRING_TYPE x v ==> no_closures v`,
-  Cases_on`x` \\ SIMP_TAC std_ss [STRING_TYPE_def,no_closures_def]);
-
-val EqualityType_thm = Q.prove(
-  `EqualityType abs <=>
-      (!x1 v1. abs x1 v1 ==> no_closures v1) /\
-      (!x1 v1 x2 v2. abs x1 v1 /\ abs x2 v2 ==> types_match v1 v2 /\
-                                                (v1 = v2 <=> x1 = x2))`,
-  SIMP_TAC std_ss [EqualityType_def] \\ METIS_TAC []);
-
-val STRING_TYPE_lemma = Q.prove(
-  `EqualityType (STRING_TYPE)`,
-  METIS_TAC (eq_lemmas ()));
-
-val EqualityType_TYPE = Q.prove(
-  `EqualityType TYPE_TYPE`,
-  SIMP_TAC std_ss [EqualityType_thm] \\ STRIP_TAC THEN1
-   (HO_MATCH_MP_TAC type_ind
-    \\ FULL_SIMP_TAC std_ss [TYPE_TYPE_def]
-    \\ REPEAT STRIP_TAC
-    \\ FULL_SIMP_TAC std_ss [no_closures_def,EVERY_DEF]
-    \\ IMP_RES_TAC (LIST_TYPE_NO_CLOSURES |> GEN_ALL)
-    \\ METIS_TAC [CHAR_IMP_no_closures,STRING_IMP_no_closures])
-  \\ HO_MATCH_MP_TAC type_ind \\ reverse STRIP_TAC THEN1
-   (REPEAT STRIP_TAC
-    \\ Cases_on `x2` \\ FULL_SIMP_TAC (srw_ss()) [TYPE_TYPE_def]
-    \\ FULL_SIMP_TAC (srw_ss()) [types_match_def,ctor_same_type_def]
-    \\ ASSUME_TAC STRING_TYPE_lemma
-    \\ FULL_SIMP_TAC std_ss [EqualityType_def] \\ RES_TAC)
-  \\ REPEAT GEN_TAC \\ STRIP_TAC \\ REPEAT GEN_TAC \\ STRIP_TAC
-  \\ Cases_on `x2` \\ FULL_SIMP_TAC (srw_ss()) [TYPE_TYPE_def]
-  \\ FULL_SIMP_TAC (srw_ss()) [types_match_def,ctor_same_type_def]
-  \\ MATCH_MP_TAC (METIS_PROVE [] ``(b1 /\ (x1 = y1)) /\ (b2 /\ (x2 = y2)) ==>
-       (b1 /\ b2) /\ ((x1 /\ x2 <=> y1 /\ y2))``)
-  \\ STRIP_TAC THEN1
-   (ASSUME_TAC STRING_TYPE_lemma
-    \\ FULL_SIMP_TAC std_ss [EqualityType_def] \\ RES_TAC
-    \\ ASM_SIMP_TAC std_ss [])
-  \\ MATCH_MP_TAC LIST_TYPE_11
-  \\ Q.EXISTS_TAC `TYPE_TYPE`
-  \\ FULL_SIMP_TAC std_ss []
-  \\ REPEAT STRIP_TAC \\ RES_TAC)
-  |> store_eq_thm;
-
-val _ = register_type ``:term``;
-val _ = register_type ``:thm``;
-val _ = register_type ``:update``;
-
-val _ = register_exn_type ``:hol_exn``;
-
-val HOL_EXN_TYPE_def = theorem"HOL_EXN_TYPE_def";
-
-(*
-  fetch "-" "TYPE_TYPE_def";
-  fetch "-" "TERM_TYPE_def";
-  fetch "-" "THM_TYPE_def";
-*)
-
-(* ref 0 *)
-
-val init_type_constants_def = Define `
-init_type_constants = [(strlit"bool",0); (strlit"fun",2:num)]`;
-
-val init_type_constants_v = translate init_type_constants_def;
-
-val e = ``(App Opref [Var (Short "init_type_constants")])``;
-				      
-val _ = ml_prog_update (add_Dlet (derive_eval_thm "the_type_constants" e) "the_type_constants" [])
-		       
-(* for debugging:
-val s = ref ml_progLib.init_state
-val _ = ml_prog_update (fn k => (s := k; k))
-val k = !s
-*)
-
-val the_type_constants_def = DB.fetch "ml_monadProg" "the_type_constants_def";
-
-(* Where is this used? *)
-(* val _ = ml_prog_update (fn k => let
-  val lemma = Q.prove(
-    `evaluate F ^(get_env k) ^(get_state k)
-        (App Opref [Var (Short "init_type_constants")])
-        (^(get_state k) with refs := init_type_constants_refs ++ [Refv init_type_constants_v],
-         Rval (the_type_constants))`,
-    ntac 5 (fs [Once evaluate_cases,PULL_EXISTS,do_app_def,store_alloc_def,
-        EVAL ``lookup_var_id (Short "init_type_constants") ^(get_env k)``])
-    \\ EVAL_TAC \\ fs [])
-    in add_Dlet lemma "the_type_constants" [the_type_constants_def] k end); *)
-
-(* ref 1 *)
-
-val init_term_constants_def = Define `
-  init_term_constants = [(strlit"=",
-    Tyapp (strlit"fun")
-      [Tyvar (strlit"A");
-       Tyapp (strlit"fun")
-         [Tyvar (strlit"A");
-          Tyapp (strlit"bool") []]])]`
-
-val init_term_constants_v = translate init_term_constants_def
-
-val e = ``(App Opref [Var (Short "init_term_constants")])``
-
-val _ = ml_prog_update (add_Dlet (derive_eval_thm "the_term_constants" e) "the_term_constants" [])
-		       
-(* for debugging:
-val s = ref ml_progLib.init_state
-val _ = ml_prog_update (fn k => (s := k; k))
-val k = !s
- *)
-
-val the_term_constants_def = DB.fetch "ml_monadProg" "the_term_constants_def";
-
-(* val _ = ml_prog_update (fn k => let
-  val lemma = Q.prove(
-    `evaluate F ^(get_env k) ^(get_state k)
-        (App Opref [Var (Short "init_term_constants")])
-        (^(get_state k) with refs := init_type_constants_refs ++ [Refv init_type_constants_v] ++
-                                     init_term_constants_refs ++ [Refv init_term_constants_v],
-         Rval (the_term_constants))`,
-    ntac 5 (fs [Once evaluate_cases,PULL_EXISTS,do_app_def,store_alloc_def,
-        EVAL ``lookup_var_id (Short "init_term_constants") ^(get_env k)``])
-    \\ EVAL_TAC \\ fs [])
-  in add_Dlet lemma "the_term_constants" [the_term_constants_def] k end) *)
-
-(* ref 2 *)
-
-val init_axioms_def = Define `
-  init_axioms = []:thm list`
-
-val init_axioms_v = translate init_axioms_def
-
-val e = ``(App Opref [Var (Short "init_axioms")])``
-
-val _ = ml_prog_update (add_Dlet (derive_eval_thm "the_axioms" e) "the_axioms" [])
-
-(* for debugging:
-val s = ref ml_progLib.init_state
-val _ = ml_prog_update (fn k => (s := k; k))
-val k = !s
- *)
-
-val the_axioms_def = DB.fetch "ml_monadProg" "the_axioms_def";
-
-(* val _ = ml_prog_update (fn k => let
-  val lemma = Q.prove(
-    `evaluate F ^(get_env k) ^(get_state k)
-        (App Opref [Var (Short "init_axioms")])
-        (^(get_state k) with refs := init_type_constants_refs ++ [Refv init_type_constants_v] ++
-                                     init_term_constants_refs ++ [Refv init_term_constants_v] ++
-                                     init_axioms_refs ++ [Refv init_axioms_v],
-         Rval (the_axioms))`,
-    ntac 5 (fs [Once evaluate_cases,PULL_EXISTS,do_app_def,store_alloc_def,
-        EVAL ``lookup_var_id (Short "init_axioms") ^(get_env k)``])
-    \\ EVAL_TAC \\ fs [])
-  in add_Dlet lemma "the_axioms" [the_axioms_def] k end) *)
-
-(* ref 3 *)
-
-val init_context_def = Define `
-  init_context = ^(rhs(concl(holSyntaxTheory.init_ctxt_def)))`
-
-val init_context_v = translate init_context_def
-
-val e = ``(App Opref [Var (Short "init_context")])``
-
-val _ = ml_prog_update (add_Dlet (derive_eval_thm "the_context" e) "the_context" [])
-
-(* for debugging:
-val s = ref ml_progLib.init_state
-val _ = ml_prog_update (fn k => (s := k; k))
-val k = !s
- *)
-
-val the_context_def = DB.fetch "ml_monadProg" "the_context_def";
-
-(* val _ = ml_prog_update (fn k => let
-  val lemma = Q.prove(
-    `evaluate F ^(get_env k) ^(get_state k)
-        (App Opref [Var (Short "init_context")])
-        (^(get_state k) with refs := init_type_constants_refs ++ [Refv init_type_constants_v] ++
-                                     init_term_constants_refs ++ [Refv init_term_constants_v] ++
-                                     init_axioms_refs ++ [Refv init_axioms_v] ++
-                                     init_context_refs ++ [Refv init_context_v],
-         Rval (the_context))`,
-    ntac 5 (fs [Once evaluate_cases,PULL_EXISTS,do_app_def,store_alloc_def,
-        EVAL ``lookup_var_id (Short "init_context") ^(get_env k)``])
-    \\ EVAL_TAC \\ fs [])
-  in add_Dlet lemma "the_context" [the_context_def] k end) *)
-
-(********************** DEPRECATED ************************************************************)
-val isRefv_def = Define `
-  isRefv P x = ?v. (x = Refv v) /\ P v`;
-
- val HOL_STORE_OLD_def = Define `
-  HOL_STORE_OLD refs s <=>
-    ∃type_constants term_constants axioms context.
-    init_type_constants_refs ++ [type_constants] ++
-    init_term_constants_refs ++ [term_constants] ++
-    init_axioms_refs ++ [axioms] ++
-    init_context_refs ++ [context] ≼ s ∧
-    isRefv ((LIST_TYPE (PAIR_TYPE STRING_TYPE NUM))
-            refs.the_type_constants) type_constants /\
-    isRefv ((LIST_TYPE (PAIR_TYPE STRING_TYPE TYPE_TYPE))
-            refs.the_term_constants) term_constants /\
-    isRefv (LIST_TYPE THM_TYPE refs.the_axioms) axioms /\
-    isRefv (LIST_TYPE UPDATE_TYPE refs.the_context) context`;
-
-(**********************************************************************************************)
-
- 
-val HOL_STORE_def = Define `
-    (HOL_STORE : hol_refs -> hprop) =
-    \refs.
-    SEP_EXISTS type_constants term_constants axioms context.
-    REF the_type_constants type_constants *
-    &(LIST_TYPE (PAIR_TYPE STRING_TYPE NUM) refs.the_type_constants type_constants) *
-    REF the_term_constants term_constants *
-    &(LIST_TYPE (PAIR_TYPE STRING_TYPE TYPE_TYPE) refs.the_term_constants term_constants) *
-    REF the_axioms axioms *
-    &(LIST_TYPE THM_TYPE refs.the_axioms axioms) *
-    REF the_context context *
-    &(LIST_TYPE UPDATE_TYPE refs.the_context context)`;
-
-(* TODO:
- Prove a theorem like: `HOL_STORE refs h ==> ?s. h = store2heap s.refs`
-*)
-
+(* REFS_PRED *)
 val REFS_PRED_def = Define `REFS_PRED H refs s = (H refs * GC) (store2heap s.refs)`;
-
+val VALID_REFS_PRED_def = Define `VALID_REFS_PRED H = ?(s : unit state) refs. REFS_PRED H refs s`;
 
 (*
  * Proof of REFS_PRED_APPEND:
@@ -342,12 +103,12 @@ last_x_assum IMP_RES_TAC >>
 fs[]);
 
 val store2heap_aux_IN_LENGTH = Q.store_thm ("store2heap_aux_IN_LENGTH",
-  `!s r x n. Mem r x IN (store2heap_aux n s) ==> r < n + LENGTH s`,
-  Induct THENL [all_tac, Cases] \\
-  fs [store2heap_aux_def] \\
-  Cases_on `r` \\ fs [] \\ rewrite_tac [ONE] \\
-  rpt strip_tac \\ fs[ADD_CLAUSES, GSYM store2heap_aux_suc] \\
-  metis_tac[]
+`!s r x n. Mem r x IN (store2heap_aux n s) ==> r < n + LENGTH s`,
+Induct THENL [all_tac, Cases] \\
+fs [store2heap_aux_def] \\
+Cases_on `r` \\ fs [] \\ rewrite_tac [ONE] \\
+rpt strip_tac \\ fs[ADD_CLAUSES, GSYM store2heap_aux_suc] \\
+metis_tac[]
 );
 
 val store2heap_aux_DISJOINT = Q.store_thm("store2heap_aux_DISJOINT",
@@ -409,10 +170,138 @@ POP_ASSUM (fn x => fs[x]) >>
 irule SPLIT_DECOMPOSWAP >>
 instantiate >> fs[store2heap_def]);
 
-(* Remove that? *)
 val REFS_PRED_append = Q.store_thm("REFS_PRED_append",
-`REFS_PRED H refs s ==> REFS_PRED H refs (s with refs := s.refs ++ junk)`,
+`!H refs s. REFS_PRED H refs s ==> REFS_PRED H refs (s with refs := s.refs ++ junk)`,
 rw[REFS_PRED_def, STORE_APPEND_JUNK]);
+
+(*
+ * Proof of STORE_EXTRACT_FROM_HPROP:
+ * `!l xv H s. (REF (Loc l) xv * H) (store2heap s) ==> ?ps. ((ps ++ [Refv xv]) ≼ s) /\ LENGTH ps = l`
+ *)
+
+val store2heap_aux_LOC_MEM = Q.store_thm("store2heap_aux_LOC_MEM",
+`!l xv H n s. (REF (Loc l) xv * H) (store2heap_aux n s) ==> Mem l (Refv xv) IN (store2heap_aux n s)`,
+rw[store2heap_aux_def] >>
+fs[STAR_def, SPLIT_def] >>
+fs[REF_def, SEP_EXISTS] >>
+fs[HCOND_EXTRACT] >>
+fs[cell_def, one_def] >>
+rw[] >>
+last_x_assum (fn x => rw[GSYM x]));
+
+val store2heap_LOC_MEM = Q.store_thm("store2heap_LOC_MEM",
+`!l xv H s. (REF (Loc l) xv * H) (store2heap s) ==> Mem l (Refv xv) IN (store2heap s)`,
+rw[store2heap_def, store2heap_aux_LOC_MEM] >> IMP_RES_TAC store2heap_aux_LOC_MEM);
+
+val isPREFIX_TAKE = Q.store_thm("isPREFIX_TAKE",
+`!l s. isPREFIX (TAKE l s) s`,
+rw[] >>
+`isPREFIX (TAKE l s) (TAKE l s ++ DROP l s)` by fs[TAKE_DROP] >>
+metis_tac[TAKE_DROP]);
+
+val isPREFIX_APPEND_EQ = Q.store_thm("isPREFIX_APPEND_EQ",
+`!a1 a2 b1 b2. LENGTH a1 = LENGTH a2 ==> (isPREFIX (a1 ++ b1) (a2 ++ b2) <=> a2 = a1 /\ isPREFIX b1 b2)`,
+Induct_on `a1` >- fs[LENGTH_NIL_SYM] >>
+rw[] >>
+Cases_on `a2` >- fs[] >>
+fs[] >> metis_tac[]);
+
+val STORE_DECOMPOS_FROM_HPROP = Q.store_thm("STORE_DECOMPOS_FROM_HPROP",
+`!l xv H s. (REF (Loc l) xv * H) (store2heap s) ==> ?ps. ((ps ++ [Refv xv]) ≼ s) /\ LENGTH ps = l`,
+rw[] >>
+IMP_RES_TAC store2heap_LOC_MEM >>
+IMP_RES_TAC store2heap_IN_EL >>
+qexists_tac `TAKE l s` >>
+Cases_on `l + 1 <= LENGTH s`
+>-(
+    fs[LENGTH_TAKE] >>
+    SUFF_TAC ``isPREFIX [Refv (xv : v)] (DROP l s)``
+    >- metis_tac[LENGTH_TAKE, LENGTH_DROP, GSYM isPREFIX_APPEND_EQ, TAKE_DROP] >>
+    FIRST_ASSUM (fn x => PURE_REWRITE_TAC[x]) >>
+    SUFF_TAC ``Refv (xv:v) = HD(DROP l s)``
+    >-( fs[] >> Cases_on `DROP l s` >- fs[DROP_NIL] >> fs[]) >>
+    fs[hd_drop]
+) >>
+irule FALSITY >>
+IMP_RES_TAC store2heap_IN_LENGTH >>
+fs[]);
+
+val STORE_EXTRACT_FROM_HPROP = Q.store_thm("STORE_EXTRACT_FROM_HPROP",
+`!l xv H s. (REF (Loc l) xv * H) (store2heap s) ==>
+!junk. EL l (s ++ junk) = Refv xv`,
+rw[] >>
+IMP_RES_TAC STORE_DECOMPOS_FROM_HPROP >>
+fs[IS_PREFIX_APPEND] >>
+first_x_assum(fn x => CONV_RULE (CHANGED_CONV (SIMP_CONV pure_ss [GSYM APPEND_ASSOC])) x |> ASSUME_TAC) >>
+`~NULL ([Refv xv] ++ (l' ++ junk))` by fs[NULL_EQ] >>
+IMP_RES_TAC EL_LENGTH_APPEND >>
+fs[HD] >>
+metis_tac[]);
+
+val SPLIT3_swap12 = Q.store_thm("SPLIT3_swap12",
+`!h h1 h2 h3. SPLIT3 h (h1, h2, h3) = SPLIT3 h (h2, h1, h3)`,
+rw[SPLIT3_def, UNION_COMM, CONJ_COMM] >> metis_tac[DISJOINT_SYM]);
+
+val SPLIT_of_SPLIT3_1u3 = Q.store_thm("SPLIT_of_SPLIT3_1u3",
+`∀h h1 h2 h3. SPLIT3 h (h1,h2,h3) ⇒ SPLIT h (h2, h1 ∪ h3)`,
+metis_tac[SPLIT3_swap12, SPLIT_of_SPLIT3_2u3]);
+
+val SEPARATE_STORE_ELEM_IN_HEAP = Q.store_thm("SEPARATE_STORE_ELEM_IN_HEAP",
+`!s0 x s1. SPLIT3 (store2heap (s0 ++ [x] ++ s1)) (store2heap s0, {Mem (LENGTH s0) x}, store2heap_aux (LENGTH s0 + 1) s1)`,
+sg `!(s0 : v store) s1 x. SPLIT (store2heap_aux (LENGTH s0) (x::s1)) ({Mem (LENGTH s0) x}, store2heap_aux (LENGTH s0 + 1) s1)`
+>-(
+    rw[store2heap_def] >>
+    PURE_REWRITE_TAC[Once rich_listTheory.CONS_APPEND] >>
+    PURE_REWRITE_TAC [GSYM (EVAL ``store2heap_aux (LENGTH (s0 : v store)) [x]``)] >>
+    ASSUME_TAC (EVAL ``LENGTH [x : v store_v]``) >>
+    metis_tac[store2heap_aux_SPLIT, ADD_COMM]
+) >>
+rw[] >>
+qspecl_then [`s0`, `[x] ++ s1`] ASSUME_TAC store2heap_SPLIT >> fs[] >>
+last_x_assum(qspecl_then [`s0`, `s1`, `x`] ASSUME_TAC) >>
+fs[SPLIT_def, SPLIT3_def] >>
+rw[]
+>-(metis_tac[UNION_ASSOC, EQ_REFL])
+>-(DISCH_TAC >> IMP_RES_TAC store2heap_IN_LENGTH >> fs[]) >>
+metis_tac[DISJOINT_UNION_BOTH, EQ_REFL]);
+
+val REF_HPROP_SAT_EQ = Q.store_thm("REF_HPROP_SAT_EQ",
+`!l xv s. REF (Loc l) xv s <=> s = {Mem l (Refv xv)}`,
+fs[REF_def, SEP_EXISTS, HCOND_EXTRACT, cell_def, one_def]);
+
+val SPLIT_UNICITY_R = Q.store_thm("SPLIT_UNICITY_R",
+`SPLIT s (u, v) ==> (SPLIT s (u, v') <=> v' = v)`,
+fs[SPLIT_EQ]);
+
+val STORE_SAT_LOC_STAR_H_EQ = Q.store_thm("STORE_SAT_LOC_STAR_H_EQ",
+`!s0 xv s1 H. (Loc (LENGTH s0) ~~> xv * H) (store2heap (s0 ++ [Refv xv] ++ s1)) <=>
+H ((store2heap s0) UNION (store2heap_aux (LENGTH s0 + 1) s1))`,
+rw[] >>
+qspecl_then [`s0`, `Refv xv`, `s1`] ASSUME_TAC SEPARATE_STORE_ELEM_IN_HEAP >>
+IMP_RES_TAC SPLIT_of_SPLIT3_1u3 >>
+last_x_assum(fn x => ALL_TAC) >>
+EQ_TAC
+>-(
+    rw[STAR_def, REF_HPROP_SAT_EQ] >>
+    IMP_RES_TAC SPLIT_UNICITY_R >>
+    fs[]
+) >>
+DISCH_TAC >>
+rw[STAR_def] >>
+instantiate >>
+rw[REF_HPROP_SAT_EQ]);
+
+val STORE_UPDATE_HPROP = Q.store_thm("STORE_UPDATE_HPROP",
+`(Loc l ~~> xv * H) (store2heap s) ==> (Loc l ~~> xv' * H) (store2heap (LUPDATE (Refv xv') l s))`,
+DISCH_TAC >>
+sg `?s0 s1. s = s0 ++ [Refv xv] ++ s1 /\ LENGTH s0 = l`
+>-(
+    IMP_RES_TAC STORE_DECOMPOS_FROM_HPROP >>
+    IMP_RES_TAC rich_listTheory.IS_PREFIX_APPEND >>
+    SATISFY_TAC
+) >>
+rw[LUPDATE_APPEND1, LUPDATE_APPEND2, LUPDATE_def] >>
+metis_tac[STORE_SAT_LOC_STAR_H_EQ, REF_HPROP_SAT_EQ, STAR_def]);
 
 (*
  * Definition of EvalM
@@ -425,28 +314,26 @@ val EvalM_def = Define `
     ?s2 res refs2. evaluate F env (s with refs := s.refs ++ junk) exp (s2,res) /\
     P (refs, s) (refs2, s2, res) /\ REFS_PRED H refs2 s2`;
 
-(* refinement invariant for ``:'a M`` *)
+(* refinement invariant for ``:('a, 'b, 'c) M`` *)
+val _ = type_abbrev("M", ``:'a -> ('b, 'c) exc # 'a``);
 
-val _ = type_abbrev("M", ``:'refs -> 'a hol_result # 'refs``);
-
-val HOL_MONAD_def = Define `
-  HOL_MONAD (a:'a->v->bool) (x:('a, 'refs) M) (state1:'refs,s1:unit state)
+val MONAD_def = Define `
+  MONAD (a:'a->v->bool) (b: 'b->v->bool) (x:('refs, 'a, 'b) M)
+                                    (state1:'refs,s1:unit state)
                                      (state2:'refs,s2:unit state,
                                       res: (v,v) result) =
     case (x state1, res) of
-      ((HolRes y, st), Rval v) => (st = state2) /\ a y v
-    | ((HolErr e, st), Rerr (Rraise v)) => (st = state2) /\
-                                              HOL_EXN_TYPE e v
+      ((Success y, st), Rval v) => (st = state2) /\ a y v
+    | ((Failure e, st), Rerr (Rraise v)) => (st = state2) /\
+                                              b e v
     | _ => F`
-
-(* Should bind and return be defined elsewhere than in holKernel ? *)
 
 (* return *)
 
 val EvalM_return = Q.store_thm("EvalM_return",
-  `!H. Eval env exp (a x) ==>
-    EvalM env exp (HOL_MONAD a (ex_return x)) H`,
-  rw[Eval_def,EvalM_def,ex_return_def,HOL_MONAD_def] \\
+  `!H b. Eval env exp (a x) ==>
+    EvalM env exp (MONAD a b (ex_return x)) H`,
+  rw[Eval_def,EvalM_def,st_ex_return_def,MONAD_def] \\
   first_x_assum(qspec_then`(s with refs := s.refs ++ junk).refs`strip_assume_tac)
   \\ IMP_RES_TAC (evaluate_empty_state_IMP
                   |> INST_TYPE [``:'ffi``|->``:unit``]) \\
@@ -457,10 +344,10 @@ val EvalM_return = Q.store_thm("EvalM_return",
 (* bind *)
 
 val EvalM_bind = Q.store_thm("EvalM_bind",
-  `!H. EvalM env e1 (HOL_MONAD b (x:('b, hol_refs) M)) H /\
-    (!x v. b x v ==> EvalM (write name v env) e2 (HOL_MONAD a ((f x):('a, hol_refs) M)) H) ==>
-    EvalM env (Let (SOME name) e1 e2) (HOL_MONAD a (ex_bind x f)) H`,
-  rw[EvalM_def,HOL_MONAD_def,ex_return_def,PULL_EXISTS] \\
+  `!H c. EvalM env e1 (MONAD b c (x:('refs, 'b, 'c) M)) H /\
+    (!x v. b x v ==> EvalM (write name v env) e2 (MONAD a c ((f x):('refs, 'a, 'c) M)) H) ==>
+    EvalM env (Let (SOME name) e1 e2) (MONAD a c (ex_bind x f)) H`,
+  rw[EvalM_def,MONAD_def,st_ex_return_def,PULL_EXISTS] \\
   first_x_assum drule \\
   disch_then(qspec_then`junk`strip_assume_tac) \\
   Cases_on`x refs` \\ Cases_on`q` \\ Cases_on`res` \\ fs[]
@@ -470,13 +357,13 @@ val EvalM_bind = Q.store_thm("EvalM_bind",
     asm_exists_tac \\ rw[] \\
     first_x_assum drule \\ disch_then drule \\
     disch_then(qspec_then`[]`strip_assume_tac) \\
-    fs[GSYM write_def,namespaceTheory.nsOptBind_def,ex_bind_def,with_same_refs] \\
+    fs[GSYM write_def,namespaceTheory.nsOptBind_def,st_ex_bind_def,with_same_refs] \\
     asm_exists_tac \\ fs[] \\ metis_tac[] )
   \\ Cases_on`e` \\ fs[] \\
   rw[Once evaluate_cases] \\
   srw_tac[DNF_ss][] \\ disj2_tac \\
   asm_exists_tac \\ rw[] \\
-  rw[ex_bind_def]);
+  rw[st_ex_bind_def]);
 
 (* lift pure refinement invariants *)
 
@@ -524,47 +411,6 @@ val evaluate_list_cases = let
           (``evaluate_list a5 a6 a7 (x::xs) (a9,Rval a10)``
            |> SIMP_CONV (srw_ss()) [Once lemma]) end
 
-(*
-val pmatch_add_refs = Q.store_thm("pmatch_add_refs",
-  `(∀cenv refs p v env.
-    pmatch cenv refs p v env ≠ Match_type_error ⇒
-    pmatch cenv (refs ++ refs') p v env = pmatch cenv refs p v env) ∧
-   (∀cenv refs ps vs env.
-    pmatch_list cenv refs ps vs env ≠ Match_type_error ⇒
-    pmatch_list cenv (refs ++ refs') ps vs env = pmatch_list cenv refs ps vs env)`,
-   ho_match_mp_tac pmatch_ind
-   \\ rw[pmatch_def]
-   \\ every_case_tac \\ fs[store_lookup_def,EL_APPEND1]
-   \\ rw[]);
-
-val do_app_add_refs = Q.store_thm("do_app_add_refs",
-  `do_app (refs,ffi) op args = SOME ((refs2,ffi2),res) ⇒
-   do_app (refs++refs',ffi) op args = SOME ((refs2++refs',ffi2),res)`,
-  rw[semanticPrimitivesPropsTheory.do_app_cases] \\
-  fs[store_alloc_def]
-  \\ rw[]
-  not true : allocating a reference adds it to the end
-
-val evaluate_add_refs = Q.store_thm("evaluate_add_refs",
-  `(∀(s:'ffi state) env es s' res.
-     evaluate s env es = (s',res) ∧ res ≠ Rerr (Rabort Rtype_error) ⇒
-     ∀refs. evaluate (s with refs := s.refs ++ refs) env es =
-            (s' with refs := s'.refs ++ refs,res)) ∧
-   (∀(s:'ffi state) env v pes errv s' res.
-     evaluate_match s env v pes errv = (s',res) ∧ res ≠ Rerr (Rabort Rtype_error) ⇒
-     ∀refs. evaluate_match (s with refs := s.refs ++ refs) env v pes errv =
-            (s' with refs := s'.refs ++ refs,res))`,
-  ho_match_mp_tac evaluate_ind
-  \\ rw[evaluate_def]
-  \\ (
-    rpt(split_pair_case_tac \\ fs[]) \\
-    rpt (
-      qpat_x_assum`_ = (s',_)`mp_tac \\
-      TOP_CASE_TAC \\ strip_tac \\ rveq \\
-      fs[] \\ rfs[pmatch_add_refs] \\ fs[] \\ rveq
-      \\ fs[evaluateTheory.dec_clock_def] ) )
-*)
-
 val EvalM_ArrowM = Q.store_thm("EvalM_ArrowM",
   `!H. EvalM env x1 ((ArrowM H a b) f) H ==>
     EvalM env x2 (a x) H ==>
@@ -611,14 +457,6 @@ val EvalM_Fun_Eq = Q.store_thm("EvalM_Fun_Eq",
   \\ first_x_assum drule \\ rw[]
   \\ first_x_assum(qspec_then `junk ++ junk'` assume_tac)
   \\ rw[] \\ SATISFY_TAC);
-
-(* Generalisation of the previous HOL_STORE_EXISTS theorem *)
-val VALID_REFS_PRED_def = Define `VALID_REFS_PRED H = ?(s : unit state) refs. REFS_PRED H refs s`;
-
-(* TODO: *)
-val HOL_STORE_EXISTS = Q.store_thm("HOL_STORE_EXISTS",
-  `VALID_REFS_PRED HOL_STORE`,
-  cheat);
 
 (* More proofs *)
 val EvalM_Fun_PURE_IMP = Q.store_thm("EvalM_Fun_PURE_IMP",
@@ -747,58 +585,12 @@ val FUN_EXISTS_Eq = Q.prove(
 val M_FUN_QUANT_SIMP = save_thm("M_FUN_QUANT_SIMP",
   LIST_CONJ [FUN_EXISTS_Eq,M_FUN_FORALL_PUSH1,M_FUN_FORALL_PUSH2]);
 
-(* failwith *)
-
-val EvalM_failwith = Q.store_thm("EvalM_failwith",
-  `!H x a.
-      (lookup_cons "Fail" env = SOME (1,TypeExn (Long "Kernel" (Short "Fail")))) ==>
-      Eval env exp1 (STRING_TYPE x) ==>
-      EvalM env (Raise (Con (SOME (Short "Fail")) [exp1]))
-        (HOL_MONAD a (failwith x)) H`,
-  rw[Eval_def,EvalM_def,HOL_MONAD_def,failwith_def] >>
-  rw[Once evaluate_cases] >>
-  rw[Once evaluate_cases] >>
-  srw_tac[boolSimps.DNF_ss][] >> disj1_tac >>
-  rw[Once evaluate_cases,PULL_EXISTS] >>
-  rw[Once(CONJUNCT2 evaluate_cases)] >>
-  first_x_assum(qspec_then`(s with refs := s.refs ++ junk).refs`strip_assume_tac) >>
-  IMP_RES_TAC (evaluate_empty_state_IMP
-               |> INST_TYPE [``:'ffi``|->``:unit``]) >>
-  rw[do_con_check_def,build_conv_def] >>
-  fs [lookup_cons_def] >>
-  fs[HOL_EXN_TYPE_def,namespaceTheory.id_to_n_def] >>
-  asm_exists_tac \\ fs[] >>
-  PURE_REWRITE_TAC[GSYM APPEND_ASSOC] \\ METIS_TAC[REFS_PRED_append]);
-
-(* clash *)
-
-val EvalM_raise_clash = Q.store_thm("EvalM_raise_clash",
-  `!H x a.
-      (lookup_cons "Clash" env = SOME (1,TypeExn (Long "Kernel" (Short "Clash")))) ==>
-      Eval env exp1 (TERM_TYPE x) ==>
-      EvalM env (Raise (Con (SOME (Short "Clash")) [exp1]))
-        (HOL_MONAD a (raise_clash x)) H`,
-  rw[Eval_def,EvalM_def,HOL_MONAD_def,raise_clash_def] >>
-  rw[Once evaluate_cases] >>
-  rw[Once evaluate_cases] >>
-  srw_tac[boolSimps.DNF_ss][] >> disj1_tac >>
-  rw[Once evaluate_cases,PULL_EXISTS] >>
-  rw[Once(CONJUNCT2 evaluate_cases)] >>
-  rw[do_con_check_def,build_conv_def] >>
-  fs [lookup_cons_def] >>
-  fs[HOL_EXN_TYPE_def,namespaceTheory.id_to_n_def] >>
-  first_x_assum(qspec_then`(s with refs := s.refs ++ junk).refs`strip_assume_tac) >>
-  IMP_RES_TAC (evaluate_empty_state_IMP
-               |> INST_TYPE [``:'ffi``|->``:unit``]) >>
-  fs[] >> asm_exists_tac \\ fs[] >>
-  PURE_REWRITE_TAC[GSYM APPEND_ASSOC] \\ METIS_TAC[REFS_PRED_append]);
-
 (* otherwise *)
 
 val EvalM_otherwise = Q.store_thm("EvalM_otherwise",
-  `!H n. EvalM env exp1 (HOL_MONAD a x1) H ==>
-        (!i. EvalM (write n i env) exp2 (HOL_MONAD a x2) H) ==>
-        EvalM env (Handle exp1 [(Pvar n,exp2)]) (HOL_MONAD a (x1 otherwise x2)) H`,
+  `!H b n. EvalM env exp1 (MONAD a b x1) H ==>
+        (!i. EvalM (write n i env) exp2 (MONAD a b x2) H) ==>
+        EvalM env (Handle exp1 [(Pvar n,exp2)]) (MONAD a b (x1 otherwise x2)) H`,
   SIMP_TAC std_ss [EvalM_def] \\ REPEAT STRIP_TAC
   \\ SIMP_TAC (srw_ss()) [Once evaluate_cases]
   \\ Q.PAT_X_ASSUM `!s refs. bb ==> bbb` (MP_TAC o Q.SPECL [`s`,`refs`])
@@ -806,10 +598,10 @@ val EvalM_otherwise = Q.store_thm("EvalM_otherwise",
   \\ first_x_assum(qspec_then`junk`strip_assume_tac)
   \\ Cases_on `res` THEN1
    (srw_tac[DNF_ss][] >> disj1_tac \\
-    asm_exists_tac \\ fs[HOL_MONAD_def,otherwise_def] \\
+    asm_exists_tac \\ fs[MONAD_def,otherwise_def] \\
     CASE_TAC \\ fs[] \\ CASE_TAC \\ fs[] )
-  \\ Q.PAT_X_ASSUM `HOL_MONAD xx yy t1 t2` MP_TAC
-  \\ SIMP_TAC std_ss [Once HOL_MONAD_def] \\ STRIP_TAC
+  \\ Q.PAT_X_ASSUM `MONAD xx yy zz t1 t2` MP_TAC
+  \\ SIMP_TAC std_ss [Once MONAD_def] \\ STRIP_TAC
   \\ Cases_on `x1 refs` \\ FULL_SIMP_TAC (srw_ss()) []
   \\ Cases_on `q` \\ FULL_SIMP_TAC (srw_ss()) [otherwise_def]
   \\ Cases_on `e` \\ FULL_SIMP_TAC (srw_ss()) [otherwise_def]
@@ -821,53 +613,10 @@ val EvalM_otherwise = Q.store_thm("EvalM_otherwise",
   \\ disch_then(qspecl_then[`v`,`[]`]strip_assume_tac)
   \\ fs[with_same_refs]
   \\ asm_exists_tac \\ fs[]
-  \\ fs[HOL_MONAD_def]
+  \\ fs[MONAD_def]
   \\ CASE_TAC \\ fs[]
   \\ CASE_TAC \\ fs[]
   \\ asm_exists_tac \\ fs[]);
-
-(* handle_clash *)
-
-val EvalM_handle_clash = Q.store_thm("EvalM_handle_clash",
-  `!H n. (lookup_cons "Clash" env = SOME (1,TypeExn (Long "Kernel" (Short "Clash")))) ==>
-        EvalM env exp1 (HOL_MONAD a x1) H ==>
-        (!t v.
-          TERM_TYPE t v ==>
-          EvalM (write n v env) exp2 (HOL_MONAD a (x2 t)) H) ==>
-        EvalM env (Handle exp1 [(Pcon (SOME (Short "Clash")) [Pvar n],exp2)])
-          (HOL_MONAD a (handle_clash x1 x2)) H`,
-  SIMP_TAC std_ss [EvalM_def] \\ REPEAT STRIP_TAC
-  \\ SIMP_TAC (srw_ss()) [Once evaluate_cases]
-  \\ Q.PAT_X_ASSUM `!s refs. REFS_PRED H refs s ==> bbb` (MP_TAC o Q.SPECL [`s`,`refs`])
-  \\ FULL_SIMP_TAC std_ss [] \\ REPEAT STRIP_TAC
-  \\ first_x_assum(qspec_then`junk`strip_assume_tac)
-  \\ Cases_on `res` THEN1
-   (srw_tac[DNF_ss][] >> disj1_tac \\
-    asm_exists_tac \\ fs[HOL_MONAD_def,handle_clash_def] \\
-    CASE_TAC \\ fs[] \\ CASE_TAC \\ fs[] )
-  \\ Q.PAT_X_ASSUM `HOL_MONAD xx yy t1 t2` MP_TAC
-  \\ SIMP_TAC std_ss [Once HOL_MONAD_def] \\ STRIP_TAC
-  \\ Cases_on `x1 refs` \\ FULL_SIMP_TAC (srw_ss()) []
-  \\ Cases_on `q` \\ FULL_SIMP_TAC (srw_ss()) [handle_clash_def]
-  \\ Cases_on `e` \\ FULL_SIMP_TAC (srw_ss()) [handle_clash_def]
-  \\ srw_tac[boolSimps.DNF_ss][] >> disj2_tac >> disj1_tac
-  \\ asm_exists_tac \\ fs[]
-  \\ simp[Once (CONJUNCT2 evaluate_cases),PULL_EXISTS,pat_bindings_def]
-  \\ Cases_on `h` >> fs[HOL_EXN_TYPE_def] >>
-  simp[pmatch_def] >> fs[lookup_cons_def] >>
-  fs[same_tid_def,namespaceTheory.id_to_n_def,same_ctor_def] >- (
-    simp[Once evaluate_cases,HOL_MONAD_def,HOL_EXN_TYPE_def] ) >>
-  first_x_assum drule >>
-  disch_then drule >>
-  simp[GSYM write_def] >>
-  disch_then(qspec_then`[]`strip_assume_tac) >>
-  fs[with_same_refs] >>
-  asm_exists_tac >>
-  fs[HOL_MONAD_def] >>
-  TOP_CASE_TAC \\ fs[] \\
-  TOP_CASE_TAC \\ fs[] \\
-  TOP_CASE_TAC \\ fs[] \\
-  TOP_CASE_TAC \\ fs[]);
 
 (* if *)
 
@@ -890,7 +639,7 @@ val EvalM_If = Q.store_thm("EvalM_If",
   \\ simp[do_if_def]
   \\ rw[]
   \\ first_x_assum (match_mp_tac o MP_CANON)
-  \\ fs[addressTheory.CONTAINER_def]);
+  \\ fs[ml_translatorTheory.CONTAINER_def]);
 
 val Eval_Var_SIMP2 = Q.store_thm("Eval_Var_SIMP2",
   `Eval (write x i env) (Var (Short y)) p =
@@ -924,7 +673,7 @@ val EvalM_PMATCH_NIL = Q.store_thm("EvalM_PMATCH_NIL",
       Eval env x (a xv) ==>
       CONTAINER F ==>
       EvalM env (Mat x []) (b (PMATCH xv [])) H`,
-  rw[addressTheory.CONTAINER_def]);
+  rw[ml_translatorTheory.CONTAINER_def]);
 
 val EvalM_PMATCH = Q.store_thm("EvalM_PMATCH",
   `!H b a x xv.
@@ -991,304 +740,46 @@ val EvalM_PMATCH = Q.store_thm("EvalM_PMATCH",
 
 (* read and update refs *)
 
-(* Proof of STORE_EXTRACT_FROM_HPROP:
-   `!l xv H s. (REF (Loc l) xv * H) (store2heap s) ==> ?ps. ((ps ++ [Refv xv]) ≼ s) /\ LENGTH ps = l`
-*)
-val HCOND_EXTRACT = cfLetAutoTheory.HCOND_EXTRACT;
-
-val store2heap_aux_LOC_MEM = Q.store_thm("store2heap_aux_LOC_MEM",
-`!l xv H n s. (REF (Loc l) xv * H) (store2heap_aux n s) ==> Mem l (Refv xv) IN (store2heap_aux n s)`,
-rw[store2heap_aux_def] >>
-fs[STAR_def, SPLIT_def] >>
-fs[REF_def, SEP_EXISTS] >>
-fs[HCOND_EXTRACT] >>
-fs[cell_def, one_def] >>
-rw[] >>
-last_x_assum (fn x => rw[GSYM x]));
-
-val store2heap_LOC_MEM = Q.store_thm("store2heap_LOC_MEM",
-`!l xv H s. (REF (Loc l) xv * H) (store2heap s) ==> Mem l (Refv xv) IN (store2heap s)`,
-rw[store2heap_def, store2heap_aux_LOC_MEM] >> IMP_RES_TAC store2heap_aux_LOC_MEM);
-
-val isPREFIX_TAKE = Q.store_thm("isPREFIX_TAKE",
-`!l s. isPREFIX (TAKE l s) s`,
-rw[] >>
-`isPREFIX (TAKE l s) (TAKE l s ++ DROP l s)` by fs[TAKE_DROP] >>
-metis_tac[TAKE_DROP]);
-
-val isPREFIX_APPEND_EQ = Q.store_thm("isPREFIX_APPEND_EQ",
-`!a1 a2 b1 b2. LENGTH a1 = LENGTH a2 ==> (isPREFIX (a1 ++ b1) (a2 ++ b2) <=> a2 = a1 /\ isPREFIX b1 b2)`,
-Induct_on `a1` >- fs[LENGTH_NIL_SYM] >>
-rw[] >>
-Cases_on `a2` >- fs[] >>
-fs[] >> metis_tac[]);
-
-val STORE_DECOMPOS_FROM_HPROP = Q.store_thm("STORE_DECOMPOS_FROM_HPROP",
-`!l xv H s. (REF (Loc l) xv * H) (store2heap s) ==> ?ps. ((ps ++ [Refv xv]) ≼ s) /\ LENGTH ps = l`,
-rw[] >>
-IMP_RES_TAC store2heap_LOC_MEM >>
-IMP_RES_TAC store2heap_IN_EL >>
-qexists_tac `TAKE l s` >>
-Cases_on `l + 1 <= LENGTH s`
->-(
-    fs[LENGTH_TAKE] >>
-    SUFF_TAC ``isPREFIX [Refv (xv : v)] (DROP l s)``
-    >- metis_tac[LENGTH_TAKE, LENGTH_DROP, GSYM isPREFIX_APPEND_EQ, TAKE_DROP] >>
-    FIRST_ASSUM (fn x => PURE_REWRITE_TAC[x]) >>
-    SUFF_TAC ``Refv (xv:v) = HD(DROP l s)``
-    >-( fs[] >> Cases_on `DROP l s` >- fs[DROP_NIL] >> fs[]) >>
-    fs[hd_drop]
-) >>
-irule FALSITY >>
-IMP_RES_TAC store2heap_IN_LENGTH >>
-fs[]);
-
-val STORE_EXTRACT_FROM_HPROP = Q.store_thm("STORE_EXTRACT_FROM_HPROP",
-`!l xv H s. (REF (Loc l) xv * H) (store2heap s) ==>
-!junk. EL l (s ++ junk) = Refv xv`,
-rw[] >>
-IMP_RES_TAC STORE_DECOMPOS_FROM_HPROP >>
-fs[IS_PREFIX_APPEND] >>
-first_x_assum(fn x => CONV_RULE (CHANGED_CONV (SIMP_CONV pure_ss [GSYM APPEND_ASSOC])) x |> ASSUME_TAC) >>
-`~NULL ([Refv xv] ++ (l' ++ junk))` by fs[NULL_EQ] >>
-IMP_RES_TAC EL_LENGTH_APPEND >>
-fs[HD] >>
-metis_tac[]);
-
-val SPLIT3_swap12 = Q.store_thm("SPLIT3_swap12",
-`!h h1 h2 h3. SPLIT3 h (h1, h2, h3) = SPLIT3 h (h2, h1, h3)`,
-rw[SPLIT3_def, UNION_COMM, CONJ_COMM] >> metis_tac[DISJOINT_SYM]);
-
-val SPLIT_of_SPLIT3_1u3 = Q.store_thm("SPLIT_of_SPLIT3_1u3",
-`∀h h1 h2 h3. SPLIT3 h (h1,h2,h3) ⇒ SPLIT h (h2, h1 ∪ h3)`,
-metis_tac[SPLIT3_swap12, SPLIT_of_SPLIT3_2u3]);
-
-val SEPARATE_STORE_ELEM_IN_HEAP = Q.store_thm("SEPARATE_STORE_ELEM_IN_HEAP",
-`!s0 x s1. SPLIT3 (store2heap (s0 ++ [x] ++ s1)) (store2heap s0, {Mem (LENGTH s0) x}, store2heap_aux (LENGTH s0 + 1) s1)`,
-sg `!(s0 : v store) s1 x. SPLIT (store2heap_aux (LENGTH s0) (x::s1)) ({Mem (LENGTH s0) x}, store2heap_aux (LENGTH s0 + 1) s1)`
->-(
-    rw[store2heap_def] >>
-    PURE_REWRITE_TAC[Once rich_listTheory.CONS_APPEND] >>
-    PURE_REWRITE_TAC [GSYM (EVAL ``store2heap_aux (LENGTH (s0 : v store)) [x]``)] >>
-    ASSUME_TAC (EVAL ``LENGTH [x : v store_v]``) >>
-    metis_tac[store2heap_aux_SPLIT, ADD_COMM]
-) >>
-rw[] >>
-qspecl_then [`s0`, `[x] ++ s1`] ASSUME_TAC store2heap_SPLIT >> fs[] >>
-last_x_assum(qspecl_then [`s0`, `s1`, `x`] ASSUME_TAC) >>
-fs[SPLIT_def, SPLIT3_def] >>
-rw[]
->-(metis_tac[UNION_ASSOC, EQ_REFL])
->-(DISCH_TAC >> IMP_RES_TAC store2heap_IN_LENGTH >> fs[]) >>
-metis_tac[DISJOINT_UNION_BOTH, EQ_REFL]);
-
-val REF_HPROP_SAT_EQ = Q.store_thm("REF_HPROP_SAT_EQ",
-`!l xv s. REF (Loc l) xv s <=> s = {Mem l (Refv xv)}`,
-fs[REF_def, SEP_EXISTS, HCOND_EXTRACT, cell_def, one_def]);
-
-val SPLIT_UNICITY_R = Q.store_thm("SPLIT_UNICITY_R",
-`SPLIT s (u, v) ==> (SPLIT s (u, v') <=> v' = v)`,
-fs[SPLIT_EQ]);
-
-val STORE_SAT_LOC_STAR_H_EQ = Q.store_thm("STORE_SAT_LOC_STAR_H_EQ",
-`!s0 xv s1 H. (Loc (LENGTH s0) ~~> xv * H) (store2heap (s0 ++ [Refv xv] ++ s1)) <=>
-H ((store2heap s0) UNION (store2heap_aux (LENGTH s0 + 1) s1))`,
-rw[] >>
-qspecl_then [`s0`, `Refv xv`, `s1`] ASSUME_TAC SEPARATE_STORE_ELEM_IN_HEAP >>
-IMP_RES_TAC SPLIT_of_SPLIT3_1u3 >>
-last_x_assum(fn x => ALL_TAC) >>
-EQ_TAC
->-(
-    rw[STAR_def, REF_HPROP_SAT_EQ] >>
-    IMP_RES_TAC SPLIT_UNICITY_R >>
-    fs[]
-) >>
-DISCH_TAC >>
-rw[STAR_def] >>
-instantiate >>
-rw[REF_HPROP_SAT_EQ]);
-
-val STORE_UPDATE_HPROP = Q.store_thm("STORE_UPDATE_HPROP",
-`(Loc l ~~> xv * H) (store2heap s) ==> (Loc l ~~> xv' * H) (store2heap (LUPDATE (Refv xv') l s))`,
-DISCH_TAC >>
-sg `?s0 s1. s = s0 ++ [Refv xv] ++ s1 /\ LENGTH s0 = l`
->-(
-    IMP_RES_TAC STORE_DECOMPOS_FROM_HPROP >>
-    IMP_RES_TAC rich_listTheory.IS_PREFIX_APPEND >>
-    SATISFY_TAC
-) >>
-rw[LUPDATE_APPEND1, LUPDATE_APPEND2, LUPDATE_def] >>
-metis_tac[STORE_SAT_LOC_STAR_H_EQ, REF_HPROP_SAT_EQ, STAR_def]);
-
-(******** TODO: move that **********************************************************************)
-fun PURE_FACTS_FIRST_CONV H =
-  let
-      val preds = list_dest dest_star H
-      val (pfl, hpl) = List.partition (can dest_pure_fact) preds
-      val ordered_preds = pfl @ hpl
-  in
-      if List.length ordered_preds = 0 then REFL H
-      else
-	  let val H' = List.foldl (fn (x, y) => mk_star(y, x)) (List.hd ordered_preds)
-				  (List.tl ordered_preds)
-          (* For some strange reason, AC_CONV doesn't work *)
-          val H_to_norm = STAR_AC_CONV H
-	  val norm_to_H' = SYM(STAR_AC_CONV H')
-	  in TRANS H_to_norm norm_to_H'
-	  end
-  end;
-
-fun pure_fact_order (t1, t2) =
-  if same_const t2 ``GC`` andalso t1 <> t2 then LESS
-  else if same_const t1 ``GC`` andalso t1 <> t2 then GREATER
-  else
-  case (is_cond t1, is_cond t2) of
-      (true, false) => LESS
-    | (false, true) => LESS
-    | _ => Term.compare(t1, t2);
-
-(* val PURE_FACTS_FIRST_CONV = sort{assoc = STAR_ASSOC, comm = STAR_COMM, dest = dest_star, mk = mk_star, cmp = pure_fact_order, combine = ALL_CONV, preprocess = ALL_CONV}; *)
-				     
-fun EXTRACT_PURE_FACTS_TAC (g as (asl, w)) =
-  let
-      fun is_hprop a = ((dest_comb a |> fst |> type_of) = ``:hprop`` handle HOL_ERR _ => false)
-      val hpreds = List.filter is_hprop asl
-      val hpreds' = List.map (fst o dest_comb) hpreds
-      val hpreds_eqs = List.map (PURE_FACTS_FIRST_CONV) hpreds'
-  in
-      ((fs hpreds_eqs) >> fs[GSYM STAR_ASSOC] >> fs[HCOND_EXTRACT] >> fs[STAR_ASSOC]) g
-  end;
-(***********************************************************************************************)
-
-(*val read_tac =
-  rw[EvalM_def]
-  \\ rw[Once evaluate_cases,evaluate_list_cases,PULL_EXISTS]
-  \\ ntac 6 (rw[Once evaluate_cases])
-  \\ fs[HOL_STORE_def,IS_PREFIX_APPEND]
-  \\ rw[do_app_def]
-  \\ fs[the_type_constants_def,the_term_constants_def,the_axioms_def,the_context_def]
-  \\ rw[store_lookup_def,EL_APPEND1,EL_APPEND2]
-  \\ fs[isRefv_def]
-  \\ srw_tac[DNF_ss][] \\ fs[]
-  \\ disj1_tac
-  \\ fs[get_the_type_constants_def,get_the_term_constants_def,get_the_axioms_def,get_the_context_def]
-  \\ fs[HOL_MONAD_def];*)
-
-val get_heap_constant_thm = Q.store_thm("get_heap_constant_thm",
-`!vname loc x TYPE H get_var.
+val EvalM_read_heap = Q.store_thm("EvalM_read_heap",
+`!vname loc x TYPE EXC_TYPE H get_var.
   nsLookup env.v (Short vname) = SOME (Loc loc) ==>
   EvalM env (App Opderef [Var (Short vname)])
-  (HOL_MONAD TYPE (λrefs. (HolRes (get_var refs), refs)))
+  (MONAD TYPE EXC_TYPE (λrefs. (Success (get_var refs), refs)))
   (λrefs. (SEP_EXISTS xv. (Loc loc) ~~> xv * &(TYPE (get_var refs) xv)) * H refs)`,
   rw[EvalM_def]
   \\ rw[Once evaluate_cases,evaluate_list_cases,PULL_EXISTS]
   \\ ntac 6 (rw[Once evaluate_cases])
-  \\ fs[REFS_PRED_def, HOL_STORE_def]
+  \\ fs[REFS_PRED_def]
   \\ fs[SEP_CLAUSES, SEP_EXISTS_THM]
   \\ EXTRACT_PURE_FACTS_TAC
   \\ fs[GSYM STAR_ASSOC]
-  \\ fs[the_type_constants_def]
   \\ rw[do_app_def]
   \\ rw[store_lookup_def,EL_APPEND1,EL_APPEND2]
   >-(
       qexists_tac `s with refs := s.refs ++ junk`
       \\ IMP_RES_TAC STORE_EXTRACT_FROM_HPROP \\ POP_ASSUM (fn x => fs[x])
       \\ fs[with_same_refs, with_same_ffi]
-      \\ fs[HOL_MONAD_def, get_the_type_constants_def]
+      \\ fs[MONAD_def]
       \\ instantiate
       \\ fs[STAR_ASSOC, STORE_APPEND_JUNK]
   ) >>
-  fs[HOL_MONAD_def, get_the_type_constants_def]
+  fs[MONAD_def] (* , get_the_type_constants_def] *)
   \\ IMP_RES_TAC store2heap_LOC_MEM
   \\ IMP_RES_TAC store2heap_IN_LENGTH
   \\ `LENGTH init_type_constants_refs >= LENGTH s.refs` by fs[]
   \\ fs[]);
 
-val SWAP_SEP_EXISTS_THM = Q.store_thm("SWAP_SEP_EXISTS_THM",
-`!H. (SEP_EXISTS u v. H u v) = (SEP_EXISTS v u. H u v)`,
-rw[SEP_EXISTS] \\
-CONV_TAC (RAND_CONV (SIMP_CONV bool_ss [Once SWAP_EXISTS_THM])) \\
-rw[]);
-
-(* Normalize the heap predicate before using the get_heap_constant_thm theorem  *)
-val SEP_EXISTS_SEPARATE_lemma = List.hd(SPEC_ALL SEP_CLAUSES |> CONJUNCTS) |> GSYM |> GEN_ALL;
-val SEP_EXISTS_INWARD_lemma = List.nth(SPEC_ALL SEP_CLAUSES |> CONJUNCTS, 1) |> GSYM |> GEN_ALL;
-
-val SEPARATE_SEP_EXISTS_CONV = ((SIMP_CONV pure_ss [GSYM STAR_ASSOC, SEP_EXISTS_INWARD_lemma])
-				    THENC (SIMP_CONV pure_ss [STAR_ASSOC, SEP_EXISTS_SEPARATE_lemma]));
-
-fun pick_sep_exists_order var (t1, t2) =
-  if is_sep_exists t1 andalso (fst o dest_sep_exists) t1 = var then LESS
-  else if is_sep_exists t2 andalso (fst o dest_sep_exists) t2 = var then GREATER
-  else Term.compare(t1, t2);
-
-fun PICK_SEP_EXISTS_CONV varname = sort{assoc = STAR_ASSOC, comm = STAR_COMM, dest = dest_star, mk = mk_star, cmp = pick_sep_exists_order (mk_var (varname, ``:v``)), combine = ALL_CONV, preprocess = ALL_CONV};
-
-fun PICK_SEP_EXISTS_TAC varname =
-  CONV_TAC(ONCE_DEPTH_CONV(ABS_CONV (SEPARATE_SEP_EXISTS_CONV THENC (PICK_SEP_EXISTS_CONV varname))));
-
-fun ABSTRACT_HEAP_READ_ACCESS get_function =
-  let  val th = (GSYM (EVAL get_function)) in
-      CONV_TAC(ONCE_DEPTH_CONV(ONCE_REWRITE_CONV [th])) end;
-
-fun ABSTRACT_HEAP_WRITE_ACCESS set_function =
-  let  val th = (GSYM (EVAL set_function)) in
-      CONV_TAC(ONCE_DEPTH_CONV(ONCE_REWRITE_CONV [th])) end;
-
-(* Make it cleaner - what should be given instead of a string? how to build the get function? *)
-fun read_tac abs_name get_fun =
-  PURE_REWRITE_TAC[HOL_STORE_def] >>
-  PURE_REWRITE_TAC[the_type_constants_def,
-		   get_the_type_constants_def,
-		   the_term_constants_def,
-		   get_the_term_constants_def,
-		   the_axioms_def,
-		   get_the_axioms_def,
-		   the_context_def,
-		   get_the_context_def] >>
-  PURE_REWRITE_TAC[GSYM STAR_ASSOC] >>
-  PICK_SEP_EXISTS_TAC abs_name >>
-  ABSTRACT_HEAP_READ_ACCESS ``^get_fun refs`` >>
-  (* TODO: replace metis_tac by a combination of matching + alpha conversion *)
-  metis_tac[get_heap_constant_thm];
-
-val get_type_constants_thm = Q.store_thm("get_the_type_constants_thm",
-  `nsLookup env.v (Short "the_type_constants") = SOME the_type_constants ==>
-    EvalM env (App Opderef [Var (Short "the_type_constants")])
-      (HOL_MONAD (LIST_TYPE (PAIR_TYPE STRING_TYPE NUM))
-                 get_the_type_constants) HOL_STORE`,  
-  read_tac "type_constants" ``\refs. refs.the_type_constants``);
-
-val get_term_constants_thm = Q.store_thm("get_the_term_constants_thm",
-  `nsLookup env.v (Short "the_term_constants") = SOME the_term_constants ==>
-    EvalM env (App Opderef [Var (Short "the_term_constants")])
-      (HOL_MONAD (LIST_TYPE (PAIR_TYPE STRING_TYPE TYPE_TYPE))
-                 get_the_term_constants) HOL_STORE`,
-  read_tac "term_constants" ``\refs. refs.the_term_constants``);
-
-val get_the_axioms_thm = Q.store_thm("get_the_axioms_thm",
-  `nsLookup env.v (Short "the_axioms") = SOME the_axioms ==>
-    EvalM env (App Opderef [Var (Short "the_axioms")])
-      (HOL_MONAD (LIST_TYPE THM_TYPE) get_the_axioms) HOL_STORE`,
-  read_tac "axioms" ``\refs. refs.the_axioms``);
-
-val get_the_context_thm = Q.store_thm("get_the_context_thm",
-  `nsLookup env.v (Short "the_context") = SOME the_context ==>
-    EvalM env (App Opderef [Var (Short "the_context")])
-      (HOL_MONAD (LIST_TYPE UPDATE_TYPE) get_the_context) HOL_STORE`,
-  read_tac "context" ``\refs. refs.the_context``);
-
-val set_heap_constant_thm = Q.store_thm("set_heap_constant_thm",
-  `!vname loc x TYPE H get_var set_var env exp.
-  (!refs x. get_var (set_var refs x) = x) ==>
-  (!refs x. H (set_var refs x) = H refs) ==>
+val EvalM_write_heap = Q.store_thm("EvalM_write_heap",
+  `!vname loc x TYPE EXC_TYPE H get_var set_var env exp.
+  (!refs x. get_var (set_var x refs) = x) ==>
+  (!refs x. H (set_var x refs) = H refs) ==>
   nsLookup env.v (Short vname) = SOME (Loc loc) ==>
   Eval env exp (TYPE x) ==>
   EvalM env (App Opassign [Var (Short vname); exp])
-  ((HOL_MONAD UNIT_TYPE) (λrefs. (HolRes (), set_var refs x)))
+  ((MONAD UNIT_TYPE EXC_TYPE) (λrefs. (Success (), set_var x refs)))
   (λrefs. (SEP_EXISTS xv. (Loc loc) ~~> xv * &(TYPE (get_var refs) xv)) * H refs)`,
   rw[]
-  \\ ASSUME_TAC (Thm.INST_TYPE [``:'a`` |-> ``:'b``, ``:'b`` |-> ``:'a``] Eval_IMP_PURE)
+  \\ ASSUME_TAC (Thm.INST_TYPE [``:'a`` |-> ``:'c``, ``:'b`` |-> ``:'a``] Eval_IMP_PURE)
   \\ POP_ASSUM IMP_RES_TAC
   \\ fs[EvalM_def] \\ rw[]
   \\ rw[Once evaluate_cases,evaluate_list_cases,PULL_EXISTS]
@@ -1302,11 +793,11 @@ val set_heap_constant_thm = Q.store_thm("set_heap_constant_thm",
   \\ asm_exists_tac \\ fs[]
   \\ fs[do_app_def]
   \\ qexists_tac `Rval (Conv NONE [])`
-  \\ qexists_tac `set_var refs x`
+  \\ qexists_tac `set_var x refs`
   \\ qexists_tac `LUPDATE (Refv v) loc (s.refs ++ junk')`
   \\ qexists_tac `s.ffi`
   \\ qpat_x_assum `P (store2heap s.refs)` (fn x => ALL_TAC)
-  \\ fs[store_assign_def,EL_APPEND1,EL_APPEND2,isRefv_def,store_v_same_type_def]
+  \\ fs[store_assign_def,EL_APPEND1,EL_APPEND2,store_v_same_type_def]
   \\ fs[SEP_CLAUSES, SEP_EXISTS_THM]
   \\ EXTRACT_PURE_FACTS_TAC
   \\ fs[GSYM STAR_ASSOC] \\ IMP_RES_TAC store2heap_LOC_MEM
@@ -1314,7 +805,7 @@ val set_heap_constant_thm = Q.store_thm("set_heap_constant_thm",
   \\ IMP_RES_TAC STORE_EXTRACT_FROM_HPROP
   \\ POP_ASSUM (qspec_then `[]` ASSUME_TAC)
   \\ fs[] \\ POP_ASSUM(fn x => ALL_TAC)
-  \\ fs[HOL_MONAD_def]
+  \\ fs[MONAD_def]
   \\ instantiate
   \\ CONV_TAC (STRIP_QUANT_CONV (RATOR_CONV PURE_FACTS_FIRST_CONV))
   \\ fs[GSYM STAR_ASSOC] \\ fs[HCOND_EXTRACT]
@@ -1322,103 +813,6 @@ val set_heap_constant_thm = Q.store_thm("set_heap_constant_thm",
   \\ IMP_RES_TAC STORE_UPDATE_HPROP
   \\ first_x_assum(qspec_then `v` ASSUME_TAC)
   \\ fs[]);
-
-fun read_tac abs_name get_fun =
-  PURE_REWRITE_TAC[HOL_STORE_def] >>
-  PURE_REWRITE_TAC[the_type_constants_def,
-		   get_the_type_constants_def,
-		   the_term_constants_def,
-		   get_the_term_constants_def,
-		   the_axioms_def,
-		   get_the_axioms_def,
-		   the_context_def,
-		   get_the_context_def] >>
-  PURE_REWRITE_TAC[GSYM STAR_ASSOC] >>
-  PICK_SEP_EXISTS_TAC abs_name >>
-  ABSTRACT_HEAP_READ_ACCESS ``^get_fun refs`` >>
-  (* TODO: replace metis_tac *)
-  metis_tac[get_heap_constant_thm];
-
-(* get_H and prove_heap_access could be made better... *)
-fun get_H w =
-  let
-      val (abs, H) = strip_imp w |> snd |> dest_comb |> snd |> dest_abs
-      val H = mk_abs (abs, dest_comb H |> snd)
-  in H end;
-
-fun prove_heap_access_thms get_fun set_fun (g as (asl, w)) =
-  let
-      val H = get_H w
-
-      (* Read access *)	    
-      val read_theorem = EVAL ``(!refs x. ^get_fun (^set_fun refs x) = x)``
-                 |> EQ_IMP_RULE |> snd |> PURE_REWRITE_RULE[IMP_CLAUSES, FORALL_SIMP]
-
-      (* Write access *)
-      val eq1 = EVAL ``^H (^set_fun refs x)``
-      val eq2 = GSYM(EVAL ``^H refs``)
-      val write_theorem = GEN_ALL(TRANS eq1 eq2)
-  in
-      ((ASSUME_TAC read_theorem) THEN (ASSUME_TAC write_theorem)) g
-  end;
-
-fun write_tac abs_name get_fun set_fun =
-  PURE_REWRITE_TAC[HOL_STORE_def] >>
-  PURE_REWRITE_TAC[the_type_constants_def,
-		   set_the_type_constants_def,
-		   the_term_constants_def,
-		   set_the_term_constants_def,
-		   the_axioms_def,
-		   set_the_axioms_def,
-		   the_context_def,
-		   set_the_context_def] >>
-  PURE_REWRITE_TAC[GSYM STAR_ASSOC] >>
-  PICK_SEP_EXISTS_TAC abs_name >>
-  ABSTRACT_HEAP_READ_ACCESS ``^get_fun refs`` >>
-  ABSTRACT_HEAP_WRITE_ACCESS ``^set_fun refs x`` >>
-  prove_heap_access_thms get_fun set_fun >>
-  (* TODO: remove the SWAP_FORALL *)
-  POP_ASSUM (fn x => ASSUME_TAC(CONV_RULE SWAP_FORALL_CONV x)) >>
-  (********************************)
-  ntac 2 DISCH_TAC >>
-  IMP_RES_TAC set_heap_constant_thm >>
-  fs[];
-
-val set_the_type_constants_thm = Q.store_thm("set_the_type_constants_thm",
-  `nsLookup env.v (Short "the_type_constants") = SOME the_type_constants ==>
-    Eval env exp (LIST_TYPE (PAIR_TYPE STRING_TYPE NUM) x) ==>
-    EvalM env (App Opassign [Var (Short "the_type_constants"); exp])
-      ((HOL_MONAD UNIT_TYPE) (set_the_type_constants x)) HOL_STORE`,
-  write_tac "type_constants"
-  ``\refs. refs.the_type_constants``
-  ``\refs x. refs with the_type_constants := x``);
-  
-val set_the_term_constants_thm = Q.store_thm("set_the_term_constants_thm",
-  `nsLookup env.v (Short "the_term_constants") = SOME the_term_constants ==>
-    Eval env exp (LIST_TYPE (PAIR_TYPE STRING_TYPE TYPE_TYPE) x) ==>
-    EvalM env (App Opassign [Var (Short "the_term_constants"); exp])
-      ((HOL_MONAD UNIT_TYPE) (set_the_term_constants x)) HOL_STORE`,
-  write_tac "term_constants"
-  ``\refs. refs.the_term_constants``
-  ``\refs x. refs with the_term_constants := x``);
-
-val set_the_axioms_thm = Q.store_thm("set_the_axioms_thm",
-  `nsLookup env.v (Short "the_axioms") = SOME the_axioms ==>
-    Eval env exp (LIST_TYPE THM_TYPE x) ==>
-    EvalM env (App Opassign [Var (Short "the_axioms"); exp])
-      ((HOL_MONAD UNIT_TYPE) (set_the_axioms x)) HOL_STORE`,
-  write_tac "axioms"
-  ``\refs. refs.the_axioms``
-  ``\refs x. refs with the_axioms := x``);
-
-val set_the_context_thm = Q.store_thm("set_the_context_thm",
-  `nsLookup env.v (Short "the_context") = SOME the_context ==>
-    Eval env exp (LIST_TYPE UPDATE_TYPE x) ==>
-    EvalM env (App Opassign [Var (Short "the_context"); exp])
-      ((HOL_MONAD UNIT_TYPE) (set_the_context x)) HOL_STORE`,
-  write_tac "context"
-  ``\refs. refs.the_context``
-  ``\refs x. refs with the_context := x``);
 
 val _ = (print_asts := true);
 
