candle/standard/cf_kernel/ml_monadStoreLib.sml
@@ -1,0 +1,504 @@
+structure ml_monadStoreLib :> ml_monadStoreLib = struct 
+
+open preamble ml_translatorTheory ml_translatorLib ml_pmatchTheory patternMatchesTheory
+open astTheory libTheory bigStepTheory semanticPrimitivesTheory
+open terminationTheory ml_progLib ml_progTheory
+open set_sepTheory cfTheory cfStoreTheory cfTacticsLib Satisfy
+open cfHeapsBaseTheory basisFunctionsLib
+open ml_monadBaseTheory ml_monadProgTheory Redblackmap AC_Sort
+
+fun ERR fname msg = mk_HOL_ERR "ml_monadProgLib" fname msg;
+
+val HCOND_EXTRACT = cfLetAutoTheory.HCOND_EXTRACT
+
+(******* COPY/PASTE from ml_monadProgScript.sml *****************************************)
+(*********** Comes from cfLetAutoLib.sml ***********************************************)	 
+(* [dest_pure_fact]
+   Deconstruct a pure fact (a heap predicate of the form &P) *)
+val set_sep_cond_tm = ``set_sep$cond : bool -> hprop``;
+fun dest_pure_fact p =
+  case (dest_term p) of
+  COMB dp =>
+    (if same_const set_sep_cond_tm (#1 dp) then (#2 dp)
+    else raise (ERR "dest_pure_fact" "Not a pure fact"))
+  | _ => raise (ERR "dest_pure_fact" "Not a pure fact");
+(***************************************************************************************)
+
+fun PURE_FACTS_FIRST_CONV H =
+  let
+      val preds = list_dest dest_star H
+      val (pfl, hpl) = List.partition (can dest_pure_fact) preds
+      val ordered_preds = pfl @ hpl
+  in
+      if List.null ordered_preds then REFL H
+      else
+	  let val H' = List.foldl (fn (x, y) => mk_star(y, x)) (List.hd ordered_preds)
+				  (List.tl ordered_preds)
+          (* For some strange reason, AC_CONV doesn't work *)
+          val H_to_norm = STAR_AC_CONV H
+	  val norm_to_H' = (SYM(STAR_AC_CONV H') handle UNCHANGED => REFL H')
+	  in TRANS H_to_norm norm_to_H'
+	  end
+  end;
+
+val EXTRACT_PURE_FACTS_CONV =
+  (RATOR_CONV PURE_FACTS_FIRST_CONV)
+  THENC (SIMP_CONV pure_ss [GSYM STAR_ASSOC])
+  THENC (SIMP_CONV pure_ss [HCOND_EXTRACT])
+  THENC (SIMP_CONV pure_ss [STAR_ASSOC]);
+
+(* TODO: use EXTRACT_PURE_FACT_CONV to rewrite EXTRACT_PURE_FACTS_TAC *)
+fun EXTRACT_PURE_FACTS_TAC (g as (asl, w)) =
+  let
+      fun is_hprop a = ((dest_comb a |> fst |> type_of) = ``:hprop`` handle HOL_ERR _ => false)
+      val hpreds = List.filter is_hprop asl
+      val hpreds' = List.map (fst o dest_comb) hpreds
+      val hpreds_eqs = List.map (PURE_FACTS_FIRST_CONV) hpreds'
+  in
+      ((fs hpreds_eqs) >> fs[GSYM STAR_ASSOC] >> fs[HCOND_EXTRACT] >> fs[STAR_ASSOC]) g
+  end;
+(***********************************************************************************************)
+(******* End of COPY/PASTE from ml_monadProgScipt.sml *****************************************)
+
+(* Create the store *)
+fun create_store refs_init_list store_hprop_name =
+  let
+      val _ = if List.null refs_init_list
+	      then raise (ERR "create_store" "need a non empty list of reference init values")
+	      else ()
+
+      (* Translate the definitions *)
+      fun create_ref (name, def) =
+	let
+	    val value_def = translate def
+	    val init_name = concl def |> dest_eq |> fst |> dest_const |> fst
+	    val init_name = stringLib.fromMLstring init_name
+	    val e = ``(App Opref [Var (Short ^init_name)])``
+	    val _ = ml_prog_update (add_Dlet (derive_eval_thm name e) name [])
+	    val ref_def = DB.fetch (current_theory()) (name ^ "_def")
+	in
+	    (value_def, ref_def)
+	end
+      val name_def_pairs = List.map (fn (n, d, _, _) => (n, d)) refs_init_list
+      val trans_results = List.map create_ref name_def_pairs
+  in
+      trans_results
+  end;
+
+(*
+val trans_results = create_store refs_init_list store_hprop_name;
+val (name, def, get_fun, set_fun) = List.hd refs_init_list;
+val refs_type = List.hd refs_init_list |> #3 |> dest_abs |> fst |> type_of;
+*)
+
+fun find_refs_access_functions refs_init_list = let
+    fun find_refs_read (name, def, get_fun, set_fun) = let
+	val (state, pair) = concl get_fun |> dest_eq |> snd |> dest_abs
+	val body = dest_pair pair |> fst |> rand
+	val refs_read = mk_abs(state, body)
+    in refs_read end
+
+    fun find_refs_write (name, def, get_fun, set_fun) = let
+	val (x, body) = concl set_fun |> dest_forall
+	val (state, pair) = dest_eq body |> snd |> dest_abs
+	val body = dest_pair pair |> snd
+	val refs_write = mk_abs(x, mk_abs(state, body))
+    in refs_write end
+
+    fun find_read_write (name, def, get_fun, set_fun) = let
+	val refs_read = find_refs_read(name, def, get_fun, set_fun)
+	val refs_write = find_refs_write(name, def, get_fun, set_fun)
+    in (name, def, get_fun, refs_read, set_fun, refs_write) end
+in List.map find_read_write refs_init_list end;
+
+(*
+val refs_init_list = find_refs_access_functions refs_init_list;
+*)
+
+fun create_store_X_hprop refs_init_list trans_results refs_type store_hprop_name =
+  let
+      (* Create the heap predicate for the store *)
+      val refs_var = mk_var("refs", refs_type)
+      val create_ref_hprop_params = zip trans_results (List.map (fn (_, _, _, x, _, _) => x) refs_init_list)
+      fun create_ref_hprop ((ref_v, ref_loc), get_f) =
+	let
+	    val (refinement_invariant, deep_const) = concl ref_v |> dest_comb
+	    val refinement_invariant = rator refinement_invariant
+	    val get_term = mk_comb (get_f, refs_var) |> BETA_CONV |> concl |> dest_eq |> snd
+	    val deep_var = mk_var((dest_const deep_const |> fst)^"'", dest_const deep_const |> snd)
+	    val ri_hprop = ``&(^refinement_invariant ^get_term ^deep_var) : hprop``
+				 
+	    val const_loc = concl ref_loc |> dest_eq |> fst
+	    val ref_hprop = ``REF ^(concl ref_loc |> dest_eq |> fst) ^deep_var``
+
+	    val hprop = mk_sep_exists(deep_var, mk_star(ref_hprop, ri_hprop))
+	in
+	    hprop
+	end
+      val hprops = List.map create_ref_hprop create_ref_hprop_params
+      val store_hprop = list_mk mk_star hprops ``emp``
+          |> SIMP_CONV bool_ss [STAR_ASSOC] |> concl |> dest_eq |> snd
+      val store_hprop = mk_abs(refs_var, store_hprop)
+      val store_hprop_var = mk_var(store_hprop_name, mk_type("fun", [refs_type, ``:hprop``]))
+      val store_hprop_def = Define `^store_hprop_var = ^store_hprop`
+  in
+      store_hprop_def
+  end;
+
+(* val store_X_hprop_def = create_store_X_hprop refs_init_list trans_results refs_type store_hprop_name; *)
+
+(* Prove that the current store satisfies the built heap predicate *)
+local
+    fun instantiate_ref_svalues trans_results (g as (asl, w)) =
+      let
+	  val (ref_vars, prop) = strip_exists w
+	  val hprops = rator prop |> list_dest dest_star
+	  val ref_consts = mapfilter (fn x => dest_sep_exists x |> snd |> dest_star |> fst |>
+              rator |> rand) hprops
+	  val ref_svalue_pairs = List.map (fn (ref_v, ref_loc) =>
+              ((fst o dest_eq o concl) ref_loc, (rand o rator o concl) ref_v)) trans_results
+	  val ref_svalue_map = Redblackmap.insertList
+              (Redblackmap.mkDict Term.compare, ref_svalue_pairs)
+
+	  val instants = List.map (fn x => Redblackmap.find (ref_svalue_map, x)) ref_consts
+	  val tac = List.foldl (fn (x, tac) => tac THEN (EXISTS_TAC x)) ALL_TAC instants
+      in
+	  tac g
+      end
+
+    fun instantiate_ref_values trans_results (g as (asl, w)) =
+      let
+	  val (ref_vars, prop) = strip_exists w
+	  val props = list_dest dest_conj prop 
+	  val props = List.take (props, List.length props -1)
+	  val ref_consts_pairs = List.map (fn x => (rand x, (rand o rator) x)) props
+	  val ref_consts_map = Redblackmap.insertList
+              (Redblackmap.mkDict Term.compare, ref_consts_pairs)
+	  val value_pairs = List.map (fn (ref_v, _) => ((rand o rator o concl) ref_v,
+              (rand o concl) ref_v)) trans_results
+	  val value_map = Redblackmap.insertList (Redblackmap.mkDict Term.compare, value_pairs)
+
+	  val init_vars = List.map (fn x => Redblackmap.find (ref_consts_map, x)) ref_vars
+	  val instants = List.map (fn x => Redblackmap.find (value_map, x)) init_vars
+	  val tac = List.foldl (fn (x, tac) => tac THEN (EXISTS_TAC x)) ALL_TAC instants
+      in
+	  tac g
+      end
+
+    val GC_INWARDS = Q.prove(`GC * A = A * GC`, SIMP_TAC std_ss [STAR_COMM])
+
+    val GC_DUPLICATE_1 = Q.prove(`A * (B * GC * C) = A * GC * (B * GC * C)`,
+				 SIMP_TAC std_ss [GSYM STAR_ASSOC, GC_INWARDS, GC_STAR_GC])
+
+    val GC_DUPLICATE_2 = Q.prove(`A * (B * GC) = A * GC * (B * GC)`,
+	ASSUME_TAC (Thm.INST [``C : hprop`` |-> ``emp : hprop``] GC_DUPLICATE_1)
+        \\ FULL_SIMP_TAC std_ss [GSYM STAR_ASSOC, SEP_CLAUSES])
+
+    val store2heap_aux_decompose_store1 = Q.prove(
+      `H (store2heap_aux n (a ++ (b ++ c))) =
+      (DISJOINT (store2heap_aux n (a ++ b)) (store2heap_aux (n + LENGTH (a ++b)) c) ==>
+      H ((store2heap_aux n (a ++ b)) UNION (store2heap_aux (n + LENGTH (a ++b)) c)))`,
+      EQ_TAC
+      >-(
+	 rw[]
+	 \\ FULL_SIMP_TAC pure_ss [GSYM APPEND_ASSOC]
+	 \\ FULL_SIMP_TAC pure_ss [store2heap_aux_append_many, ADD_ASSOC]
+	 \\ metis_tac[UNION_COMM, UNION_ASSOC]
+      )
+      \\ rw[]
+      \\ qspecl_then [`n`, `a ++ b`, `c`] ASSUME_TAC store2heap_aux_DISJOINT \\ fs[]
+      \\ PURE_REWRITE_TAC [Once store2heap_aux_append_many]
+      \\ fs[UNION_COMM])
+
+    val store2heap_aux_decompose_store2 = Q.prove(
+      `H (store2heap_aux n (a ++ b)) =
+      (DISJOINT (store2heap_aux n a) (store2heap_aux (n + LENGTH a) b) ==>
+      H ((store2heap_aux (n + LENGTH a) b) UNION (store2heap_aux n a)))`,
+      ASSUME_TAC (Thm.INST [``b:v store`` |-> ``[] : v store``] store2heap_aux_decompose_store1
+         |> GEN_ALL)
+      \\ fs[UNION_COMM])
+
+    val SAT_GC = Q.prove(`!h. GC h`, rw[GC_def, SEP_EXISTS] \\ qexists_tac `\x. T` \\ rw[])
+
+    val store2heap_REF_SAT = Q.prove(`((Loc l) ~~> v) (store2heap_aux l [Refv v])`,
+        fs[store2heap_aux_def] >> fs[REF_def, SEP_EXISTS_THM, HCOND_EXTRACT, cell_def, one_def])
+in
+    fun prove_valid_store_X_hprop trans_results refs_type store_X_hprop_def =
+      let
+	  val store_hprop_const = concl store_X_hprop_def |> dest_eq |> fst
+	  val current_state = get_state(get_ml_prog_state())
+	  val current_store = ``^current_state.refs``
+	  val store_eval_thm = EVAL current_store
+
+	  val goal = ``?refs. REFS_PRED ^store_hprop_const refs ^current_state``
+
+	  val solve_first_subheap_tac =
+	    PURE_REWRITE_TAC[GSYM APPEND_ASSOC]
+	    \\ PURE_ONCE_REWRITE_TAC [store2heap_aux_decompose_store1]
+	    \\ DISCH_TAC \\ PURE_ONCE_REWRITE_TAC[STAR_def] \\ BETA_TAC
+	    \\ PURE_REWRITE_TAC [SPLIT_def] \\ instantiate
+	    \\ POP_ASSUM (fn x => ALL_TAC)
+	    \\ CONJ_TAC
+	    >-(
+	       PURE_ONCE_REWRITE_TAC [store2heap_aux_decompose_store2]
+	       \\ DISCH_TAC \\ PURE_ONCE_REWRITE_TAC[STAR_def] \\ BETA_TAC
+	       \\ PURE_REWRITE_TAC [SPLIT_def]
+	       \\ PURE_ONCE_REWRITE_TAC[DISJOINT_SYM] \\ instantiate
+	       \\ SIMP_TAC std_ss [UNION_COMM, SAT_GC]
+	       \\ PURE_REWRITE_TAC (List.map snd trans_results)
+	       \\ rw[store2heap_REF_SAT]
+	    )
+
+	  fun rec_solve_subheaps_tac g =
+	    FIRST[solve_first_subheap_tac >> rec_solve_subheaps_tac, ALL_TAC] g
+
+	  val solve_tac =
+	    FULL_SIMP_TAC (srw_ss()) [REFS_PRED_def, store_X_hprop_def, store_eval_thm]
+	    \\ srw_tac[QI_ss][]
+	    \\ instantiate_ref_svalues trans_results
+	    \\ SIMP_TAC bool_ss [SEP_CLAUSES, SEP_EXISTS_THM]
+	    \\ (CONV_TAC o STRIP_QUANT_CONV) EXTRACT_PURE_FACTS_CONV
+	    \\ instantiate_ref_values trans_results
+	    \\ SIMP_TAC (bool_ss) (List.map fst trans_results)
+	    \\ SIMP_TAC pure_ss [GSYM STAR_ASSOC]
+	    \\ PURE_REWRITE_TAC [Once GC_DUPLICATE_2]
+	    \\ ntac (List.length trans_results - 2) (ONCE_REWRITE_TAC [GC_DUPLICATE_1])
+	    \\ PURE_REWRITE_TAC [store2heap_def]
+	    \\ rec_solve_subheaps_tac
+	    \\ PURE_REWRITE_TAC [Once store2heap_aux_decompose_store2]
+	    \\ DISCH_TAC \\ PURE_REWRITE_TAC[Once STAR_def] \\ BETA_TAC
+	    \\ PURE_REWRITE_TAC [SPLIT_def]
+	    \\ PURE_REWRITE_TAC[Once DISJOINT_SYM] \\ instantiate
+	    \\ SIMP_TAC std_ss [UNION_COMM, SAT_GC]
+	    \\ PURE_REWRITE_TAC (List.map snd trans_results)
+	    \\ rw[store2heap_REF_SAT]
+
+	  val thm_name = "INIT_" ^(dest_const store_hprop_const |> fst) 
+	  val store_X_hprop_thm = store_thm(thm_name, goal, solve_tac)
+	  val _ = print ("Saved theorem __ \"" ^thm_name ^"\"\n")
+      in
+	  store_X_hprop_thm
+      end
+end;
+
+(* val valid_store_X_hprop_thm = prove_valid_store_X_hprop trans_results refs_type store_X_hprop_def; *)
+
+(* Prove the validity theorem for the characteristic heap predicate *)
+fun prove_exists_store_X_hprop refs_type store_hprop_name valid_store_X_hprop_thm =
+  let
+      val store_hprop_const = mk_const(store_hprop_name, mk_type("fun", [refs_type, ``:hprop``]))
+      val current_state = get_state(get_ml_prog_state())
+      val ty_subst = Type.match_type (type_of current_state) ``:unit state``
+      val current_state = Term.inst ty_subst current_state
+      val goal = ``VALID_REFS_PRED ^store_hprop_const``
+
+      val solve_tac = 
+          PURE_REWRITE_TAC[VALID_REFS_PRED_def]
+          \\ EXISTS_TAC current_state
+          \\ SIMP_TAC std_ss [valid_store_X_hprop_thm]
+
+      val thm_name = store_hprop_name ^"_EXISTS"
+      val exists_store_X_hprop_thm = store_thm(thm_name, goal, solve_tac)
+      val _ = print ("Saved theorem __ \"" ^thm_name ^"\"\n")
+  in
+      exists_store_X_hprop_thm
+  end;
+
+(* val exists_store_X_hprop_thm = prove_exists_store_X_hprop refs_type store_hprop_name valid_store_X_hprop_thm; *)
+
+(* Prove the specifications for the get/set functions *)
+
+local
+    (* Normalize the heap predicate before using the get_heap_constant_thm theorem  *)
+    val SEP_EXISTS_SEPARATE_lemma = List.hd(SPEC_ALL SEP_CLAUSES |> CONJUNCTS) |> GSYM |> GEN_ALL
+    val SEP_EXISTS_INWARD_lemma = List.nth(SPEC_ALL SEP_CLAUSES |> CONJUNCTS, 1) |> GSYM |> GEN_ALL
+
+    val SEPARATE_SEP_EXISTS_CONV = ((SIMP_CONV pure_ss [GSYM STAR_ASSOC, SEP_EXISTS_INWARD_lemma])
+				    THENC (SIMP_CONV pure_ss [STAR_ASSOC, SEP_EXISTS_SEPARATE_lemma]))
+
+    fun pick_sep_exists_order varname (t1, t2) = let
+	val get_var_name = fst o dest_const o rand o rator o fst o dest_star
+            o snd o dest_sep_exists in
+	if is_sep_exists t1 andalso get_var_name t1 = varname then LESS
+	else if is_sep_exists t2 andalso get_var_name t2 = varname then GREATER
+	else Term.compare(t1, t2) end
+
+    fun PICK_SEP_EXISTS_CONV varname = AC_Sort.sort{assoc = STAR_ASSOC, comm = STAR_COMM, dest = dest_star, mk = mk_star, cmp = pick_sep_exists_order varname, combine = ALL_CONV, preprocess = ALL_CONV}
+
+    fun PICK_SEP_EXISTS_TAC varname =
+      CONV_TAC(ONCE_DEPTH_CONV(ABS_CONV (SEPARATE_SEP_EXISTS_CONV THENC (PICK_SEP_EXISTS_CONV varname))))
+
+    fun ABSTRACT_HEAP_READ_ACCESS_CONV get_function tm = let
+	val ref_var = strip_imp tm |> snd |> rand |> dest_abs |> fst
+	val rw_th = (GSYM (EVAL (mk_comb(get_function, ref_var))))
+    in PURE_ONCE_REWRITE_CONV [rw_th] tm end
+    
+    fun ABSTRACT_HEAP_WRITE_ACCESS (g as (asl, w)) = let
+	val x = (rand o rand o rand o rator o rand) w
+	val (refs, pair_tm) = (dest_abs o rand o rand o rator o rand o rand) w
+	val (tml, tmr) = dest_pair pair_tm
+	val tmr' = mk_abs(x, mk_abs(refs, tmr))
+	val tmr' = mk_comb(mk_comb(tmr', x), refs)
+	val rw_thm = ((RATOR_CONV BETA_CONV) THENC BETA_CONV) tmr' |> GSYM
+    in CONV_TAC(ONCE_REWRITE_CONV [rw_thm]) g end
+
+    fun ABSTRACT_HEAP_PRED_TAC (g as (asl, w)) = let
+	val tm = strip_imp w |> snd |> rand
+	val (abs, H) = dest_abs tm
+	val (H1, H2) = dest_star H
+	val rw_rule = mk_comb (mk_abs(abs, H2), abs) |> BETA_CONV |> GSYM
+    in PURE_ONCE_REWRITE_TAC [rw_rule] g end
+
+    fun prove_heap_access_thms get_fun set_fun (g as (asl, w)) =
+      let
+	  (* Read access *)	    
+	  val read_theorem = EVAL ``(!refs x. ^get_fun (^set_fun x refs) = x)``
+              |> EQ_IMP_RULE |> snd |> PURE_REWRITE_RULE[IMP_CLAUSES, FORALL_SIMP]
+
+	  (* Write access *)
+	  val H = strip_imp w |> snd |> rand |> dest_abs |> snd |>
+			    dest_star |> snd |> rator
+	  val x = mk_var("x", type_of set_fun |> dest_type |> snd |> List.hd)
+	  val refs = mk_var("refs", type_of set_fun |> dest_type |> snd |> List.last |> dest_type |> snd |> List.hd)
+	  val eq1 = EVAL ``^H (^set_fun ^x ^refs)``
+	  val eq2 = GSYM(EVAL (mk_comb(H, refs)))
+	  val write_theorem = TRANS eq1 eq2 |> GENL[refs, x]
+      in
+	  ((ASSUME_TAC read_theorem) THEN (ASSUME_TAC write_theorem)) g
+      end
+in
+
+fun prove_store_access_specs refs_init_list trans_results store_X_hprop_def refs_type exc_ri = let
+    val store_pred = concl store_X_hprop_def |> dest_eq |> fst
+    val exc_type = type_of exc_ri |> dest_type |> snd |> List.hd
+    val exc_type_aq = ty_antiq exc_type
+    val refs_type_aq = ty_antiq refs_type
+
+    (* val (name, init_def, get_fun_def, read_fun, set_fun_def, write_fun) = List.hd refs_init_list
+       val (value_def, loc_def) = List.hd trans_results
+     *)
+    fun prove_get_spec ((name, init_def, get_fun_def, read_fun, set_fun_def, write_fun),
+			(value_def, loc_def)) = let
+	val name_tm = stringLib.fromMLstring name
+	val loc_const = concl loc_def |> dest_eq |> fst
+	val ri_pred = concl value_def |> rator |> rator
+	val result_type = type_of ri_pred |> dest_type |> snd |> List.hd
+	val monad_type = ``:(^refs_type, ^result_type, ^exc_type) M``
+
+	val monad_get_fun_def = get_fun_def
+	val monad_get_fun = concl monad_get_fun_def |> dest_eq |> fst
+
+	val MONAD_RI = ``MONAD ^ri_pred ^exc_ri``
+        val tys = Type.match_type (type_of MONAD_RI |> dest_type |> snd |> List.hd) monad_type
+	val MONAD_RI = Term.inst tys MONAD_RI
+
+	val tys = Type.match_type (type_of monad_get_fun) monad_type
+	val monad_get_fun = Term.inst tys monad_get_fun
+	val goal = 
+          ``nsLookup env.v (Short ^name_tm) = SOME ^loc_const ==>
+            EvalM env (App Opderef [Var (Short ^name_tm)])
+            (^MONAD_RI ^monad_get_fun) ^store_pred``
+
+       (* set_goal([], goal) *)
+       val read_tac =
+	 PURE_REWRITE_TAC[store_X_hprop_def]
+	 \\ PURE_REWRITE_TAC[GSYM STAR_ASSOC]
+	 \\ PICK_SEP_EXISTS_TAC (dest_const loc_const |> fst)
+	 \\ PURE_REWRITE_TAC[loc_def, monad_get_fun_def]
+	 \\ CONV_TAC (ABSTRACT_HEAP_READ_ACCESS_CONV read_fun)
+	 \\ ABSTRACT_HEAP_PRED_TAC
+	 \\ PURE_REWRITE_TAC[EvalM_read_heap]
+
+	val thm_name = "get_" ^name ^"_thm"
+	val get_spec = store_thm(thm_name, goal, read_tac)
+	val _ = print ("Saved theorem __ \"" ^thm_name ^"\"\n")
+    in get_spec end
+
+    val get_specsl = List.map prove_get_spec (zip refs_init_list trans_results)
+
+    (* val (name, init_def, get_fun_def, read_fun, set_fun_def, write_fun) = List.hd refs_init_list
+       val (value_def, loc_def) = List.hd trans_results
+     *)
+    fun prove_set_spec  ((name, init_def, get_fun_def, read_fun, set_fun_def, write_fun),
+			(value_def, loc_def)) = let
+	val name_tm = stringLib.fromMLstring name
+	val loc_const = concl loc_def |> dest_eq |> fst
+	val ri_pred = concl value_def |> rator |> rator
+	val monad_type = ``:(^refs_type, unit, ^exc_type) M``
+
+	val monad_set_fun_def = set_fun_def
+	val monad_set_fun = concl monad_set_fun_def |> dest_forall |> snd |> dest_eq |> fst |> rator
+
+	val MONAD_RI = ``MONAD UNIT_TYPE ^exc_ri``
+	val tys = Type.match_type (type_of MONAD_RI |> dest_type |> snd |> List.hd) monad_type
+	val MONAD_RI = Term.inst tys MONAD_RI
+
+	val tys = Type.match_type (type_of monad_set_fun |> dest_type |> snd |> List.last) monad_type
+	val monad_set_fun = Term.inst tys monad_set_fun
+
+	val goal = 
+          ``nsLookup env.v (Short ^name_tm) = SOME ^loc_const ==>
+            Eval env exp (^ri_pred x) ==>
+            EvalM env (App Opassign [Var (Short ^name_tm); exp])
+            (MONAD UNIT_TYPE ^exc_ri (^monad_set_fun x)) ^store_pred``
+
+       (* set_goal([], goal) *)
+       val write_tac =
+	 PURE_REWRITE_TAC[store_X_hprop_def]
+	 \\ PURE_REWRITE_TAC[GSYM STAR_ASSOC]
+	 \\ PICK_SEP_EXISTS_TAC (dest_const loc_const |> fst)
+	 \\ PURE_REWRITE_TAC[loc_def, monad_set_fun_def]
+	 \\ CONV_TAC ((RAND_CONV o RAND_CONV) (ABSTRACT_HEAP_READ_ACCESS_CONV read_fun))
+	 \\ ABSTRACT_HEAP_WRITE_ACCESS
+	 \\ ABSTRACT_HEAP_PRED_TAC
+	 \\ prove_heap_access_thms read_fun write_fun
+	 \\ rpt DISCH_TAC
+	 \\ IMP_RES_TAC(Thm.INST_TYPE [``:'b`` |-> exc_type] EvalM_write_heap)
+	 \\ POP_ASSUM(fn x => PURE_REWRITE_TAC[x])
+	 
+       val thm_name = "set_" ^name ^"_thm"
+       val set_spec = store_thm(thm_name, goal, write_tac)
+       val _ = print ("Saved theorem __ \"" ^thm_name ^"\"\n")
+    in set_spec end
+
+    val set_specsl = List.map prove_set_spec (zip refs_init_list trans_results)
+in
+    (get_specsl, set_specsl)
+end
+
+end
+
+type store_translation_result =
+    {init_values_thms : thm list,
+     locations_thms  : thm list,
+     store_pred_def : thm,
+     store_pred_validity : thm,
+     store_pred_exists_thm : thm,
+     get_specs : thm list,
+     set_specs : thm list};
+
+fun mk_store_translation_result values locs pred pred_valid pred_exists gets sets =
+   ({init_values_thms = values,
+     locations_thms  = locs,
+     store_pred_def = pred,
+     store_pred_validity = pred_valid,
+     store_pred_exists_thm = pred_exists,
+     get_specs = gets,
+     set_specs = sets} : store_translation_result);
+
+fun translate_store refs_init_list store_hprop_name exc_ri = let
+    val trans_results = create_store refs_init_list store_hprop_name
+    val refs_type = List.hd refs_init_list |> #3 |> concl |> rand |> dest_abs |> fst |> type_of
+    val refs_init_list = find_refs_access_functions refs_init_list
+
+    val store_X_hprop_def = create_store_X_hprop refs_init_list trans_results refs_type store_hprop_name
+    val valid_store_X_hprop_thm = prove_valid_store_X_hprop trans_results refs_type store_X_hprop_def
+    val exists_store_X_hprop_thm = prove_exists_store_X_hprop refs_type store_hprop_name
+                                   valid_store_X_hprop_thm
+    val (get_specs, set_specs) = prove_store_access_specs refs_init_list trans_results
+                           store_X_hprop_def refs_type exc_ri
+
+    val (values, locs) = unzip trans_results
+in mk_store_translation_result values locs store_X_hprop_def valid_store_X_hprop_thm exists_store_X_hprop_thm get_specs set_specs end;
+
+end
