candle/standard/cf_kernel/ml_monad_translatorLib.sml
@@ -1,27 +1,31 @@
+structure ml_monad_translatorLib = struct
+
 open preamble
 open astTheory libTheory semanticPrimitivesTheory bigStepTheory
      ml_translatorTheory ml_translatorLib ml_progTheory ml_progLib
      ml_pmatchTheory holKernelTheory ml_monadBaseTheory ml_monadProgTheory
 open terminationTheory
-open ml_monadStoreLib ml_hol_kernelStoreProgTheory
-
-val _ = new_theory "ml_hol_kernelProg";
+open ml_monadStoreLib
 
 val RW = REWRITE_RULE;
 val RW1 = ONCE_REWRITE_RULE;
 
 val _ = (print_asts := true);
 
-val _ = translation_extends "ml_hol_kernelStoreProg"
-
 val _ = (use_full_type_names := false);
 
 (* PROVISIONAL *)
-val _ = type_abbrev("M", ``:'a -> ('b, 'c) exc # 'a``);
+(* val _ = type_abbrev("M", ``:'a -> ('b, 'c) exc # 'a``); *)
+
+(* fun dest_monad_type ty =
+  let val s = (match_type ``:('a, 'b, 'c) M`` ty) in
+      (type_subst s ``:'a``, type_subst s ``:'b``, type_subst s ``:'c``) end; *)
+
 (* END OF PROVISIONAL *)
 
+val polymorph_monad_type = ``:'a -> ('b, 'c) exc # 'a``;
 fun dest_monad_type ty =
-  let val s = (match_type ``:('a, 'b, 'c) M`` ty) in
+  let val s = (match_type polymorph_monad_type ty) in
       (type_subst s ``:'a``, type_subst s ``:'b``, type_subst s ``:'c``) end;
 
 (* Should be moved somewhere else *)
@@ -41,18 +45,6 @@ fun D th = let
 
 val env_tm = mk_var("env",semanticPrimitivesSyntax.mk_environment semanticPrimitivesSyntax.v_ty)
 
-(* Theorems, predicates and types valid for the current translation *)
-(* val H = ``HOL_STORE``;
-val refs_type = type_of H |> dest_type |> snd |> List.hd;
-fun M_type ty = ``:(hol_refs, ^ty, hol_exn) M``;
-val aM = ty_antiq (M_type ``:'a``);
-val bM = ty_antiq (M_type ``:'b``);
-
-val VALID_STORE_THM = HOL_STORE_EXISTS;
-val EXN_TYPE = ``HOL_EXN_TYPE``;
-val exn_type = type_of EXN_TYPE |> dest_type |> snd |> List.hd
-val additional_theories = ["ml_hol_kernelStoreProg"]; *)
-
 (* The store predicate *) 
 val H = ref ``\refs. emp``;
 
@@ -64,7 +56,7 @@ val EXN_TYPE = ref ``UNIT_TYPE``;
 val exn_type = ref ``:unit``;
 
 (* Some functions to generate monad types *)
-fun M_type ty = ``:(^(!refs_type), ^ty, ^(!exn_type)) M``;
+fun M_type ty = ``:^(!refs_type) -> (^ty, ^(!exn_type)) exc # ^(!refs_type)``;
 val aM = ref (ty_antiq (M_type ``:'a``));
 val bM = ref (ty_antiq (M_type ``:'b``));
 
@@ -72,14 +64,18 @@ val bM = ref (ty_antiq (M_type ``:'b``));
 val VALID_STORE_THM = ref (prove(``T``, fs[]));
 
 (* Additional theories where to look for refinement invariants *)
-val additional_theories = ref ([] : string list);
+val type_theories = ref ([current_theory(), "ml_translator"] : string list);
 
 (* Theorems proved by the user to handle exceptions *)
-val custom_patterns = ref ([] : thm list);
+val exn_handles = ref ([] : (term * thm) list);
+val exn_raises = ref ([] : (term * thm) list);
 
+(* The information about the access functions *)
+val read_refs = ref ([] : (term * term * thm) list);
+val write_refs = ref ([] : (term * term * thm) list);
 
 (* Initialize the translation by giving the appropriate values to the above references *)
-fun init_translation (store_trans_res : store_translation_result) custom_patterns type_theories =
+fun init_translation (store_trans_res : store_translation_result) exn_thms add_type_theories =
   let
       val {init_values_thms = init_values_thms,
 	   locations_thms  = locations_thms,
@@ -88,88 +84,85 @@ fun init_translation (store_trans_res : store_translation_result) custom_pattern
 	   store_pred_exists_thm = store_pred_exists_thm,
 	   get_specs = get_specs,
 	   set_specs = set_specs} = store_trans_res
-      val _ = (H := concl store_pred_def |> des_eq |> fst)
-      val _ = (refs_type := dest_type (!H) |> snd |> List.hd)
-      val _ = (EXN_TYPE := List.hd get_specs |> concl |> dest_imp |> snd |> rator |> rand |> rator |> rator)
-      val _ = (aM := (ty_antiq (M_type ``:'a``)))
-      val _ = (bM := (ty_antiq (M_type ``:'b``)))
-      val _ = (VALID_STORE_THM := store_pred_exists_thm)
-      val _ = (additional_theories := type_theories)
-      val _ = (custom_patterns := custom_patterns)
+      val _ = H := (concl store_pred_def |> dest_eq |> fst)
+      val _ = refs_type := (type_of (!H) |> dest_type |> snd |> List.hd)
+      val _ = EXN_TYPE := (List.hd get_specs |> concl |> dest_imp |> snd |> rator |> rand |> rator |> rand)
+      val _ = exn_type := (type_of (!EXN_TYPE) |> dest_type |> snd |> List.hd)
+      val _ = aM := (ty_antiq (M_type ``:'a``))
+      val _ = bM := (ty_antiq (M_type ``:'b``))
+      val _ = VALID_STORE_THM := store_pred_exists_thm
+      val _ = type_theories := (current_theory()::(add_type_theories@["ml_translator"]))
+
+      (* Exceptions *)
+      fun is_exc_raise_thm th =
+          (List.length (concl th |> strip_forall |> snd |> strip_imp |> fst) = 2)
+      val (raise_thms, handle_thms) = List.partition is_exc_raise_thm exn_thms
+      fun extract_pattern th = let
+	  val pat = concl th |> strip_forall |> snd |> strip_imp |> snd |> rator |> rand |> rand
+      in (pat, th) end
+      val _ = exn_raises := (List.map extract_pattern raise_thms)
+      val _ = exn_handles := (List.map extract_pattern handle_thms)
+
+      (* Access functions *)
+      fun get_read_info (location_thm, get_spec) = let
+	  val get_fun = concl get_spec |> rand |> rator |> rand |> rand
+	  val loc = concl location_thm |> dest_eq |> fst
+      in (get_fun, loc, get_spec) end
+      val get_funs_info = zip locations_thms get_specs
+      val _ = read_refs := (List.map get_read_info get_funs_info)
+
+      fun get_write_info (location_thm, set_spec) = let
+	  val set_fun = concl set_spec |> rand |> rand |> rator |> rand |> rand
+	  val loc = concl location_thm |> dest_eq |> fst
+      in (set_fun, loc, set_spec) end
+      val set_funs_info = zip locations_thms set_specs
+      val _ = write_refs := (List.map get_write_info set_funs_info)
   in () end;
 
-val t= (1 |-> 2)
-val {redex = x, residue = y} = t;
-
-val spec = ``nsLookup env.v (Short ^name_tm) = SOME ^loc_const ==>
-            EvalM env (App Opderef [Var (Short ^name_tm)])
-            (^MONAD_RI ^monad_get_fun) ^store_pred``
-
-type store_translation_thms =
-    {init_values_thms : thm list,
-     locations_thms  : thm list,
-     store_pred_def : thm,
-     store_pred_validity : thm,
-     store_pred_exist_thm : thm,
-     get_specs : thm list,
-     set_specs : thm list};
-
-fun mk_store_translation_thms values locs pred pred_valid pred_exists gets sets =
-   ({init_values_thms = values,
-     locations_thms  = locs,
-     store_pred_def = pred,
-     store_pred_validity = pred_valid,
-     store_pred_exist_thm = pred_exists,
-     get_specs = gets,
-     set_specs = sets} : store_translation_thms);
-
-val ISPEC_EvalM = ISPEC (!H);
-val ISPEC_EvalM_MONAD = ISPECL[!H, !EXN_TYPE];
+fun ISPEC_EvalM th = ISPEC (!H) th handle HOL_ERR _ =>  SPEC (!H) th;
+fun ISPEC_EvalM_EXN_TYPE th = ISPEC (!EXN_TYPE) th handle HOL_ERR _ =>  SPEC (!EXN_TYPE) th;
+fun ISPEC_EvalM_MONAD th = ISPEC_EvalM th |> ISPEC_EvalM_EXN_TYPE;
 
 fun inst_monad_type tm =
   let
-      val ty_subst = Type.match_type ``:('a, 'b, 'c) M`` (type_of tm)
+      val ty_subst = Type.match_type polymorph_monad_type (type_of tm)
       val a = Type.type_subst ty_subst ``:'a``
       val c = Type.type_subst ty_subst ``:'c``
-      val tm' = Term.inst [a |-> refs_type, c |-> exn_type] tm
+      val tm' = Term.inst [a |-> !refs_type, c |-> !exn_type] tm
   in
       tm'
   end;
 (* ---- *)
 
 (* ---- *)
-(* TODO: move HOL_MONAD_tm *)
-val MONAD_POLY_tm = ``MONAD : ('a -> v -> bool) -> ('b -> v -> bool) -> (('refs, 'a, 'b) M, 'refs) H``;
-val MONAD_tm = Term.inst [``:'refs`` |-> refs_type] MONAD_POLY_tm;
 fun get_m_type_inv ty =
   let
-      val monad_type = dest_monad_type ty |> #2
-      val MONAD_tm' = Term.inst [``:'a`` |-> monad_type, ``:'b`` |-> exn_type] MONAD_tm
+      val result_type = dest_monad_type ty |> #2
+      val MONAD_type = M_type result_type
+      val MONAD_RI = mk_const("MONAD", MONAD_type)
   in
-      ``^MONAD_tm' ^(get_type_inv monad_type) ^EXN_TYPE``
+      ``^MONAD_RI ^(get_type_inv result_type) ^(!EXN_TYPE)``
   end
   handle HOL_ERR _ => failwith "unknown type";
 
-val PURE_tm = ``PURE : ('a -> v -> bool) -> ('a, 'b) H``;
 fun mk_PURE_tm ty = let
-  val PURE_tm' = Term.inst [``:'a`` |-> ty, ``:'b`` |-> refs_type] PURE_tm
-  in mk_comb (PURE_tm', get_type_inv ty) end;
+  val PURE_tm = mk_const("PURE", ``:(^ty -> v -> bool) -> (^ty, ^(!refs_type)) H``)
+  in mk_comb (PURE_tm, get_type_inv ty) end;
 
 fun get_arrow_type_inv ty =
   if can dest_monad_type ty then get_m_type_inv ty else let
     val (ty1,ty2) = dest_fun_type ty
     val i1 = get_arrow_type_inv ty1 handle HOL_ERR _ =>
              mk_PURE_tm ty1
-             (* ``PURE ^(get_type_inv ty1)`` *)
     val i2 = get_arrow_type_inv ty2
-    in ``ArrowM ^H ^i1 ^i2`` end
+  in ``ArrowM ^(!H) ^i1 ^i2`` end;
 
 fun smart_get_type_inv ty =
   if not (can dest_monad_type ty) andalso
      can get_arrow_type_inv ty then let
     val inv = get_arrow_type_inv ty
     in ONCE_REWRITE_CONV [ArrowM_def] inv |> concl |> rand |> rand end
-  else get_type_inv ty
+  else get_type_inv ty;
 
 (* Retrieves the parameters given to Eval or EvalM *)
 val Eval_tm = ``Eval``;
@@ -187,21 +180,6 @@ fun remove_Eval_storePred e = if same_const (strip_comb e |> fst) Eval_tm then e
 (* support for datatypes... *)
 
 (*
-val ty = ``:'b # 'c``; val th = derive_case_of ty;
-val ty = ``:'a list``; val th = derive_case_of ty;
-val ty = ``:type``; val th = derive_case_of ty;
-val ty = ``:term``; val th = derive_case_of ty;
-val ty = ``:thm``; val th = derive_case_of ty;
-val ty = ``:update``; val th = derive_case_of ty;
-*)
-
-(******************************************************************************************
- *
- * Pattern matching
- *
- ******************************************************************************************)
-
-(*
   val _ = set_goal([],goal)
 *)	      
 fun derive_case_of ty = let
@@ -211,18 +189,17 @@ fun derive_case_of ty = let
   fun get_name ty = clean_uppercase (smart_full_name_of_type ty) ^ "_TYPE"
   val name = get_name ty
   val inv_def = tryfind (fn thy_name => fetch thy_name (name ^ "_def"))
-                        (current_theory()::(additional_theories@ [(*"ml_monadProg",*) "ml_translator"]))
+                        (!type_theories)
   val case_th = get_nchotomy_of ty
 (*
   val tm = ``Eval (write n1_2 v1_2 (write n1_1 v1_1 env)) exp1
       (return_type (f1 x1_1 x1_2))``
 *)
   val pat = ``Eval env exp (P (res:'a))``
-  (* TODO: Add support for H, add type of refs in `'a M` *)
   fun Eval_to_EvalM tm = let
     val (m,i) = match_term pat tm
     val res = mk_var("res", M_type ``:'a``)
-    val tm1 = subst m (inst i ``EvalM env exp (MONAD P ^EXN_TYPE ^res) ^H``)
+    val tm1 = subst m (inst i ``EvalM env exp (MONAD P ^(!EXN_TYPE) ^res) ^(!H)``)
     val ty1 = tm |> rand |> rand |> type_of
     val monad_ret_type = M_type ty1(* type_subst [``:'a`` |-> ty1] monad_type1 *)
     val y1 = tm |> rand |> rand |> inst [ty1|->monad_ret_type]
@@ -242,6 +219,12 @@ fun derive_case_of ty = let
   val (x3,x4) = dest_imp x3
   (* val tm = last hyps |> strip_forall |> snd |> dest_imp |> snd *)
   val hyps = list_dest dest_conj x3
+  (*
+  val f = Eval_to_EvalM;
+  val xs = List.last hyps;
+  val tm = xs;
+  val tm = strip_forall xs |> snd |> dest_imp |> snd;
+  *)
   fun map_tl f [] = []
     | map_tl f (x::xs) = x :: map f xs
   val z3 = map_tl Eval_to_EvalM hyps |> list_mk_conj
@@ -303,18 +286,13 @@ fun type_mem f = let
 
 val mem_derive_case_of = type_mem derive_case_of;
 
-val ty = ``:'b # 'c``; val _ = mem_derive_case_of ty;
+(* val ty = ``:'b # 'c``; val _ = mem_derive_case_of ty;
 val ty = ``:'a list``; val _ = mem_derive_case_of ty;
 val ty = ``:'a option``; val _ = mem_derive_case_of ty;
 val ty = ``:type``; val _ = mem_derive_case_of ty;
 val ty = ``:term``; val _ = mem_derive_case_of ty;
 val ty = ``:thm``; val _ = mem_derive_case_of ty;
-val ty = ``:update``; val _ = mem_derive_case_of ty;
-
-(*
-val tm = ``case l of [] => ex_return F | x::l' => ex_return T``;
-inst_case_thm_for tm;
-*)
+val ty = ``:update``; val _ = mem_derive_case_of ty; *)
 
 fun inst_case_thm_for tm = let
   val (_,_,names) = TypeBase.dest_case tm
@@ -357,11 +335,6 @@ fun inst_case_thm_for tm = let
 (*
 val tm = (!last_fail)
 val tm = rhs
-val original_tm = tm
-val tm = dest_conj hyps |> snd |> strip_forall |> snd |> dest_imp |> snd |> rator |> rand |> rand |> rand |> strip_abs |> snd |> rand
-val tm = ``st_ex_return v1``
-
-val tm = dest_conj hyps |> snd
 *)
 fun inst_case_thm tm m2deep = let
   val tm = if can dest_monad_type (type_of tm) then (inst_monad_type tm) else tm
@@ -416,10 +389,6 @@ fun inst_case_thm tm m2deep = let
 
 val IMP_EQ_T = Q.prove(`a ==> (a <=> T)`,fs [])
 
-(* DEBUG *)
-val prove_EvalMPatBind_fail = ref T;
-(* END DEBUG *)
-
 fun prove_EvalMPatBind goal m2deep = let
   val (vars,rhs_tm) = repeat (snd o dest_forall) goal
                       |> rand |> get_Eval_arg |> rator
@@ -465,14 +434,7 @@ fun prove_EvalMPatBind goal m2deep = let
     \\ TRY (first_x_assum match_mp_tac >> METIS_TAC[])
     \\ fs[GSYM FORALL_PROD]
     \\ EVAL_TAC)
-  in UNDISCH_ALL th end handle HOL_ERR e =>
-  (prove_EvalMPatBind_fail := goal;
-   failwith "prove_EvalMPatBind failed");
-
-(* DEBUG *)
-val pmatch_m2deep_fail = ref T;
-val tm = !pmatch_m2deep_fail;
-(* END DEBUG *)
+  in UNDISCH_ALL th end handle HOL_ERR e => failwith "prove_EvalMPatBind failed";
 
 fun pmatch_m2deep tm m2deep = let
   val (x,ts) = dest_pmatch_K_T tm
@@ -484,13 +446,13 @@ fun pmatch_m2deep tm m2deep = let
   val pmatch_inv = get_m_type_inv pmatch_type
   val x_exp = x_res |> UNDISCH |> concl |> rator |> rand
   val nil_lemma = EvalM_PMATCH_NIL
-		  |> ISPEC H
+		  |> ISPEC_EvalM
                   |> ISPEC pmatch_inv
                   |> ISPEC x_exp
                   |> ISPEC v
                   |> ISPEC x_inv
   val cons_lemma = EvalM_PMATCH
-		   |> ISPEC H
+		   |> ISPEC_EvalM
                    |> ISPEC pmatch_inv
                    |> ISPEC x_inv
                    |> ISPEC x_exp
@@ -531,8 +493,7 @@ fun pmatch_m2deep tm m2deep = let
   val th = MATCH_MP th (UNDISCH x_res)
   val th = UNDISCH_ALL th
   in th end handle HOL_ERR e =>
-  (pmatch_m2deep_fail := tm;
-   failwith ("pmatch_m2deep failed (" ^ #message e ^ ")"));
+  failwith ("pmatch_m2deep failed (" ^ #message e ^ ")");
 
 (* ---- *)
 
@@ -562,56 +523,11 @@ fun inst_EvalM_env v th = let
                |> DISCH new_assum
   in th1 end;
 
-(*
-val v = List.hd l
-val fix = true
-apply_EvalM_Fun (List.hd l) th true
-*)
-(* MATCH_MP th1 th2 fails when:
-   th1 = `!y. (!x. P x y) ==> Q
-   th2 = `!x. P x (f x)`
-   because of name conflicts.
-   MATCH_MP_ABS_RENAME renames the abstractions in th1 to prevent that from happening.
- *)
-(* fun MATCH_MP_FORALL_RENAME th1 th2 =
-  let
-      val th1_hyp = ISPEC H EvalM_Fun_Eq |> concl |> dest_imp |> fst |> strip_forall |> snd
-      (* val (quant_vars, th1_spec_hyp) = strip_forall th1_hyp *)
-      val (tms, tys) = match_term th1_hyp (concl th2);
-      val fvs = FVL (concl (SPEC_ALL th2)::(List.map (fn {redex = _, residue = x} => x) tms)) empty_varset
-      val fvl = HOLset.listItems fvs
-
-      fun rename_foralls_conv fvl tm =
-	if is_forall tm then let
-	    val (x, tm') = dest_forall tm
-  	    val x' = variant fvl x
-	    val conv_f = RAND_CONV ((ABS_CONV (rename_foralls_conv (x'::fvl))) THENC (ALPHA_CONV x'))
-	in
-	    conv_f tm
-	end
-	else REFL tm
-      val ren_th1 = CONV_RULE ((RATOR_CONV o RAND_CONV) (rename_foralls_conv fvl)) th1
-      val subst_th1 = Thm.INST tms (Thm.INST_TYPE tys ren_th1)
-  in
-      MP subst_th1 th2
-  end*)
-
 fun apply_EvalM_Fun v th fix = let
   val th1 = inst_EvalM_env v th
-  val th2 = if fix then MATCH_MP (ISPEC H EvalM_Fun_Eq) (GEN ``v:v`` th1)
-                   else MATCH_MP (ISPEC H EvalM_Fun) (GEN ``v:v`` (FORCE_GEN v th1))
+  val th2 = if fix then MATCH_MP (ISPEC_EvalM EvalM_Fun_Eq) (GEN ``v:v`` th1)
+                   else MATCH_MP (ISPEC_EvalM EvalM_Fun) (GEN ``v:v`` (FORCE_GEN v th1))
   in th2 end;
-
-(* val th1 = (ISPEC H EvalM_Fun_Eq);
-val th2 = (GEN ``v:v`` (inst_EvalM_env v th));
-MATCH_MP_FORALL_RENAME (ISPEC H EvalM_Fun_Eq) (GEN ``v:v`` (inst_EvalM_env v th)) *)
-
-(*
-apply_EvalM_Recclosure fname v th
-
-type_of inv
-type_of v
-*)
 
 fun apply_EvalM_Recclosure fname v th = let
   val vname = fst (dest_var v)
@@ -640,7 +556,7 @@ fun apply_EvalM_Recclosure fname v th = let
   val th1 = thx |> UNDISCH_ALL
                 |> CONV_RULE ((RATOR_CONV o RAND_CONV o RAND_CONV) (UNBETA_CONV v)) (* RATOR_CONV *)
                 |> DISCH new_assum
-  val th2 = MATCH_MP (ISPEC H EvalM_Recclosure) (Q.INST [`env`|->`cl_env`] (GEN ``v:v`` th1))
+  val th2 = MATCH_MP (ISPEC_EvalM EvalM_Recclosure) (Q.INST [`env`|->`cl_env`] (GEN ``v:v`` th1))
   val assum = ASSUME (fst (dest_imp (concl th2)))
   val th3 = D th2 |> REWRITE_RULE [assum]
   val lemma = MATCH_MP Eval_Eq_Recclosure assum
@@ -652,8 +568,6 @@ fun apply_EvalM_Recclosure fname v th = let
   in th4 end;
 
 (* Copy-paste from ml_translatorLib *)
-(* check_inv "failwith" tm result DEBUG
-val name = "failwith" *)
 val check_inv_fail = ref T;
 
 fun check_inv name tm result = let
@@ -668,11 +582,10 @@ fun check_inv name tm result = let
     val _ = print "\n\n\n"
     val _ = (show_types_verbosely := false)
     in failwith("checkinv") end end
-
 (* end of copy-paste *)
 				   
-(* ---- *)
 
+(* ---- *) 
 fun var_hol2deep tm =
   if is_var tm andalso can get_arrow_type_inv (type_of tm) then let
     val (name,ty) = dest_var tm
@@ -683,31 +596,11 @@ fun var_hol2deep tm =
     in check_inv "var" tm result end
   else hol2deep tm;
 
-(* TODO: automate *)
-val read_refs =
-  [(``get_the_type_constants``,``the_type_constants``,get_the_type_constants_thm),
-   (``get_the_term_constants``,``the_term_constants``,get_the_term_constants_thm),
-   (``get_the_axioms``,``the_axioms``,get_the_axioms_thm),
-   (``get_the_context``,``the_context``,get_the_context_thm)];
-
-val write_refs =
-  [(``set_the_type_constants x``,``the_type_constants``,set_the_type_constants_thm),
-   (``set_the_term_constants x``,``the_term_constants``,set_the_term_constants_thm),
-   (``set_the_axioms x``,``the_axioms``,set_the_axioms_thm),
-   (``set_the_context x``,``the_context``,set_the_context_thm)];
+(* raise, handle *)
+fun get_pattern patterns tm = tryfind (fn(pat, th) => if can (match_term pat) tm then (pat, th) else failwith "get_pattern") patterns;
 
 (*
 val tm = rhs
-val tm = !last_m2deep_tm
-*)
-
-(* DEBUG *)
-val last_m2deep_tm = ref ``T``;
-(* END DEBUG *)
-
-(*
-val tm = x1
-val tm = f
 *)
 
 (* DEBUG *)
@@ -715,21 +608,6 @@ fun print_tm_msg msg tm =
   print (msg  ^(term_to_string tm) ^ "\n\n");
 (* END DEBUG *)
 
-(*
-val tm = rhs
-val tm = ``v5 : 'b -> 'a holKernel$M``
-val tm = ``list_CASE l (ex_return 128) (\x y. ex_return 256)``
-val tm = z
-val tm = concl def |> dest_forall |> snd |> rand |> rand |> dest_abs |> snd |> rator |> rator
-val tm = ``raise_clash v1 : term holKernel$M``
-
-match_term ``(st_ex_return x): ^aM`` tm
-dest_type (type_of tm)
-val tm = ``(st_ex_return v1) : 'b holKernelPmatch$M``
- *)
-
-(* val tm = map_term; *)
-exception BREAKPOINT of term;
 
 fun m2deep tm =
   (* variable *)
@@ -740,13 +618,39 @@ fun m2deep tm =
     val inv = ONCE_REWRITE_CONV [ArrowM_def] inv |> concl |> rand |> rand
     val str = stringSyntax.fromMLstring name
     val result = ASSUME (mk_comb(``Eval env (Var (Short ^str))``,mk_comb(inv,tm)))
-    val result = MATCH_MP (ISPEC H Eval_IMP_PURE) result |> RW [GSYM ArrowM_def]
+    val result = MATCH_MP (ISPEC_EvalM Eval_IMP_PURE) result |> RW [GSYM ArrowM_def]
     in check_inv "var" tm result end else
+  (* raise *)
+  if can (get_pattern (!exn_raises)) tm then let
+    val _ = print_tm_msg "raise custom pattern\n" tm (* DEBUG *)
+    val (_, EvalM_th) = get_pattern (!exn_raises) tm
+    val ty = dest_monad_type (type_of tm)
+    val inv = smart_get_type_inv (#2 ty)
+    val th = hol2deep (rand tm)
+    val asms = List.mapPartial (Lib.total DECIDE) (hyp th)
+    val th = List.foldl (Lib.uncurry PROVE_HYP) th asms
+    val result = ISPEC_EvalM EvalM_th |> SPEC (rand tm) |> ISPEC inv
+                 |> UNDISCH |> Lib.C MATCH_MP th
+    in check_inv "raise custom pattern" tm result end else
+  (* handle *)
+  if can (get_pattern (!exn_handles)) tm then let
+    val _ = print_tm_msg "handle custom pattern\n" tm (* DEBUG *)
+    val (_, EvalM_th) = get_pattern (!exn_handles) tm
+    val x = tm |> rator |> rand
+    val (v,y) = tm |> rand |> dest_abs
+    val th1 = m2deep x
+    val th2 = m2deep y
+    val th3 = inst_EvalM_env v th2 |> Q.GEN`v` |> FORCE_GEN v
+    val lemma = ISPEC_EvalM EvalM_th |> SPEC_ALL |> UNDISCH
+    val th4 = MATCH_MP lemma th1
+    val result = MATCH_MP th4 th3 handle HOL_ERR _ => HO_MATCH_MP th4 th3
+    in check_inv "handle custom pattern" tm result end
+  (*
   (* failwith *)
   if can (match_term ``(failwith s): ^aM``) tm then let
     val _ = print_tm_msg "failwith\n" tm (* DEBUG *)
     val ty = dest_monad_type (type_of tm)
-    val inv = smart_get_type_inv (#2 ty) (* fst ty *)
+    val inv = smart_get_type_inv (#2 ty)
     val th = hol2deep (rand tm)
     val asms = List.mapPartial (Lib.total DECIDE) (hyp th)
     val th = List.foldl (Lib.uncurry PROVE_HYP) th asms
@@ -757,19 +661,36 @@ fun m2deep tm =
   if can (match_term ``(raise_clash t): ^aM``) tm then let
     val _ = print_tm_msg "raise clash\n" tm (* DEBUG *)
     val ty = dest_monad_type (type_of tm)
-    val inv = smart_get_type_inv (#2 ty) (* fst ty *)
+    val inv = smart_get_type_inv (#2 ty)
     val th = hol2deep (rand tm)
+    (* TEST *)
+    val asms = List.mapPartial (Lib.total DECIDE) (hyp th)
+    val th = List.foldl (Lib.uncurry PROVE_HYP) th asms
+    (* TEST *)
     val result = ISPEC_EvalM EvalM_raise_clash |> SPEC (rand tm) |> ISPEC inv
                  |> UNDISCH |> Lib.C MATCH_MP th
-    in check_inv "raise_clash" tm result end
+  in check_inv "raise_clash" tm result end
+  (* handle_clash *)
+  else if can (match_term ``handle_clash (x: ^aM) y``) tm then let
+    val _ = print_tm_msg "handle clash\n" tm (* DEBUG *)
+    val x = tm |> rator |> rand
+    val (v,y) = tm |> rand |> dest_abs
+    val th1 = m2deep x
+    val th2 = m2deep y
+    val th3 = inst_EvalM_env v th2 |> Q.GEN`v` |> FORCE_GEN v
+    val lemma = ISPEC_EvalM EvalM_handle_clash |> SPEC_ALL |> UNDISCH
+    val th4 = MATCH_MP lemma th1
+    val result = MATCH_MP th4 th3 handle HOL_ERR _ => HO_MATCH_MP th4 th3
+    in check_inv "handle_clash" tm result end
+  *)
   (* return *)
-  else if can (match_term ``(st_ex_return x): ^aM``) tm then let
+  else if can (match_term ``(st_ex_return x): ^(!aM)``) tm then let
     val _ = print_tm_msg "return\n" tm (* DEBUG *)
     val th = hol2deep (rand tm)
     val result = MATCH_MP (ISPEC_EvalM_MONAD EvalM_return) th
     in check_inv "return" tm result end
   (* bind *)
-  else if can (match_term ``(st_ex_bind (x:^bM) f): ^aM``) tm then let
+  else if can (match_term ``(st_ex_bind (x:^(!bM)) f): ^(!aM)``) tm then let
     val _ = print_tm_msg "bind\n" tm (* DEBUG *)
     val x1 = tm |> rator |> rand
     val (v,x2) = tm |> rand |> dest_abs
@@ -781,7 +702,7 @@ fun m2deep tm =
     val result = MATCH_MP (ISPEC_EvalM_MONAD EvalM_bind) (CONJ th1 th2)
     in check_inv "bind" tm result end else
   (* otherwise *)
-  if can (match_term ``(x: ^aM) otherwise (y: ^aM)``) tm then let
+  if can (match_term ``(x: ^(!aM)) otherwise (y: ^(!aM))``) tm then let
     val _ = print_tm_msg "otherwise\n" tm (* DEBUG *)
     val x = tm |> rator |> rand
     val y = tm |> rand
@@ -798,20 +719,8 @@ fun m2deep tm =
     val lemma = Q.SPEC `"v"` (ISPEC_EvalM_MONAD EvalM_otherwise)
     val result = MATCH_MP (MATCH_MP lemma th1) th2
     in check_inv "otherwise" tm result end else
-  (* handle_clash *)
-  if can (match_term ``handle_clash (x: ^aM) y``) tm then let
-    val _ = print_tm_msg "handle clash\n" tm (* DEBUG *)
-    val x = tm |> rator |> rand
-    val (v,y) = tm |> rand |> dest_abs
-    val th1 = m2deep x
-    val th2 = m2deep y
-    val th3 = inst_EvalM_env v th2 |> Q.GEN`v` |> FORCE_GEN v
-    val lemma = ISPEC H EvalM_handle_clash |> SPEC_ALL |> UNDISCH
-    val th4 = MATCH_MP lemma th1
-    val result = MATCH_MP th4 th3 handle HOL_ERR _ => HO_MATCH_MP th4 th3
-    in check_inv "handle_clash" tm result end else
   (* try *)
-  if can (match_term ``try (f:'a-> ^bM) x msg``) tm then let
+  if can (match_term ``try (f:'a-> ^(!bM)) x msg``) tm then let
     val _ = print_tm_msg "try\n" tm (* DEBUG *)
     val lemma = tm |> SIMP_CONV (srw_ss()) [try_def]
     val th = m2deep (lemma |> concl |> rand)
@@ -842,7 +751,7 @@ fun m2deep tm =
     val th2 = th2 |> GEN ``v:v``
     val z = th1 |> concl |> rand |> rand
     val th2 = INST [v|->z] th2
-    val result = MATCH_MP (ISPEC H EvalM_Let) (CONJ th1 th2)
+    val result = MATCH_MP (ISPEC_EvalM EvalM_Let) (CONJ th1 th2)
     in check_inv "let" tm result end else
   (* data-type pattern-matching *)
   (print_tm_msg "data-type pattern-matching\n" tm (* DEBUG *); inst_case_thm tm m2deep) handle HOL_ERR _ =>
@@ -854,29 +763,29 @@ fun m2deep tm =
     val target = mk_comb(inv,tm)
     val (ss,ii) = match_term (th |> concl |> rand) target
     val result = INST ss (INST_TYPE ii th)
-                 |> MATCH_MP (ISPEC H Eval_IMP_PURE)
+                 |> MATCH_MP (ISPEC_EvalM Eval_IMP_PURE)
                  |> REWRITE_RULE [GSYM ArrowM_def]
     in check_inv "lookup_v_thm" tm result end else
   (* if *)
-  if can (match_term ``if b then x: ^aM else y: ^aM``) tm then let
+  if can (match_term ``if b then x: ^(!aM) else y: ^(!aM)``) tm then let
     val _ = print_tm_msg "if\n" tm (* DEBUG *)
     val (t,x1,x2) = dest_cond tm
     val th0 = hol2deep t
     val th1 = m2deep x1
     val th2 = m2deep x2
-    val th = MATCH_MP (ISPEC H EvalM_If) (LIST_CONJ [D th0, D th1, D th2])
+    val th = MATCH_MP (ISPEC_EvalM EvalM_If) (LIST_CONJ [D th0, D th1, D th2])
     val result = UNDISCH th
     in check_inv "if" tm result end else
   (* ref: get_the_(...) *)
-  if can (first (fn (t,_,_) => same_const t tm)) read_refs then let
+  if can (first (fn (t,_,_) => same_const t tm)) (!read_refs) then let
     val _ = print_tm_msg "ref get_the(...)\n" tm (* DEBUG *)
-    val (_,t,result) = first (fn (t,_,_) => same_const t tm) read_refs
+    val (_,t,result) = first (fn (t,_,_) => same_const t tm) (!read_refs)
     val result = result |> UNDISCH_ALL
     in check_inv "get" tm result end else
   (* ref: set_the_(...) *)
-  if can (first (fn (t,_,_) => can (match_term t) tm)) write_refs then let
+  if can (first (fn (t,_,_) => can (match_term t) tm)) (!write_refs) then let
     val _ = print_tm_msg "ref: set_the(...)\n" tm (* DEBUG *)
-    val (_,t,result) = (first (fn (t,_,_) => can (match_term t) tm)) write_refs
+    val (_,t,result) = (first (fn (t,_,_) => can (match_term t) tm)) (!write_refs)
     val th = result |> UNDISCH
     val result = MATCH_MP th (hol2deep (tm |> rand))
     in check_inv "set" tm result end else
@@ -893,9 +802,9 @@ fun m2deep tm =
       val inv = smart_get_type_inv inv_type
       val eq = ``Eq ^inv ^tm``
       (* TODO: move that *)
-      val PURE_tm = Term.inst [``:'a`` |-> inv_type, ``:'b`` |-> refs_type] ``PURE : ('a -> v -> bool) -> ('a, 'b) H``
+      val PURE_tm = Term.inst [``:'a`` |-> inv_type, ``:'b`` |-> !refs_type] ``PURE : ('a -> v -> bool) -> ('a, 'b) H``
       in ``^PURE_tm (Eq ^inv ^tm)`` end
-    fun mk_m_arrow x y = ``ArrowM ^H ^x ^y``
+    fun mk_m_arrow x y = ``ArrowM ^(!H) ^x ^y``
     fun mk_inv [] res = res
       | mk_inv (x::xs) res = mk_inv xs (mk_m_arrow (mk_fix x) res)
 (*
@@ -908,17 +817,17 @@ val ty = type_of tm
     val pre = T (* subst ss (rec_pre_var ()) *)
     val tys = match_type (type_of f) (type_of inv |> dest_type |> snd |> List.hd)
     val f' = Term.inst tys f
-    val h = ASSUME ``PreImp ^pre (EvalM env (Var (Short ^str)) (^inv ^f') ^H)``
+    val h = ASSUME ``PreImp ^pre (EvalM env (Var (Short ^str)) (^inv ^f') ^(!H))``
             |> RW [PreImp_def] |> UNDISCH
 (*
 val original_tm
 val tm = List.last xs
 *)
-    val ys = map (fn tm => MATCH_MP (ISPEC H Eval_IMP_PURE)
+    val ys = map (fn tm => MATCH_MP (ISPEC_EvalM Eval_IMP_PURE)
                              (MATCH_MP Eval_Eq (var_hol2deep tm))) xs
     fun apply_arrow hyp [] = hyp
       | apply_arrow hyp (x::xs) =
-          MATCH_MP (MATCH_MP (ISPEC H EvalM_ArrowM) (apply_arrow hyp xs)) x
+          MATCH_MP (MATCH_MP (ISPEC_EvalM EvalM_ArrowM) (apply_arrow hyp xs)) x
           (* MATCH_MP (MATCH_MP EvalM_ArrowM (apply_arrow hyp xs)) x *)
     val result = apply_arrow h ys
     in check_inv "rec_pattern" tm result end else
@@ -936,31 +845,21 @@ val tm = List.last xs
     val _ = print_tm_msg "normal function application\n" tm (* DEBUG *)
     val (f,x) = dest_comb tm
     val thf = m2deep f
-    val result = hol2deep x |> MATCH_MP (ISPEC H Eval_IMP_PURE)
-                            |> MATCH_MP (MATCH_MP (ISPEC H EvalM_ArrowM) thf)
+    val result = hol2deep x |> MATCH_MP (ISPEC_EvalM Eval_IMP_PURE)
+                            |> MATCH_MP (MATCH_MP (ISPEC_EvalM EvalM_ArrowM) thf)
                  handle e =>
-                 m2deep x |> MATCH_MP (MATCH_MP (ISPEC H EvalM_ArrowM) thf)
+                 m2deep x |> MATCH_MP (MATCH_MP (ISPEC_EvalM EvalM_ArrowM) thf)
     in check_inv "comb" tm result end else
-  (last_m2deep_tm := tm; failwith ("cannot translate: " ^ term_to_string tm));
+  failwith ("cannot translate: " ^ term_to_string tm);
 
 fun get_curr_prog_state () = let
   val k = ref init_state
   val _ = ml_prog_update (fn s => (k := s; s))
   in !k end
 
-(*
-val def = FST;
-val def = !last_def;
-val def = map_def;
-val assoc_conv_tm = th |> concl |> rand |> rator |> rand
-*)
 fun EvalM_P_CONV CONV tm =
   if is_imp tm then (RAND_CONV o RATOR_CONV o RAND_CONV) CONV tm
   else (RATOR_CONV o RAND_CONV) CONV tm;
-
-(* DEBUG *)
-val last_def = ref assoc_def;
-(* END DEBUG *)
 
 (* Performs a conversion of the form: (\x. M x) = M *)
 (* fun ABS_PREDICATE_CONV tm =
@@ -974,9 +873,6 @@ val last_def = ref assoc_def;
 				 
 fun m_translate def = let
   val original_def = def
-  (* DEBUG *)
-  val _ = (last_def := original_def)			 
-  (* END DEBUG *)
   fun the (SOME x) = x | the _ = failwith("the of NONE")
   (* perform preprocessing -- reformulate def *)
   val (is_rec,defs,ind) = preprocess_def def
@@ -1081,12 +977,12 @@ fun m_translate def = let
                   |> clean_assumptions |> DISCH_ALL
                   |> REWRITE_RULE [GSYM AND_IMP_INTRO] |> UNDISCH_ALL
       val th = th |> DISCH (first (can (match_term ``LOOKUP_VAR _ _ _``)) (hyp th))
-      val th = MATCH_MP (MP (ISPEC H LOOKUP_VAR_EvalM_IMP) VALID_STORE_THM) (Q.GEN `env` th) (* HERE!! *)
+      val th = MATCH_MP (MP (ISPEC_EvalM LOOKUP_VAR_EvalM_IMP) (!VALID_STORE_THM)) (Q.GEN `env` th)
       in th end
     else let
       val th = th |> Q.INST [`env`|->`^(get_env (get_curr_prog_state ()))`]
                   |> D |> clean_assumptions |> UNDISCH_ALL
-      val th = th |> MATCH_MP (MP (ISPEC H EvalM_Fun_PURE_IMP) VALID_STORE_THM)
+      val th = th |> MATCH_MP (MP (ISPEC_EvalM EvalM_Fun_PURE_IMP) (!VALID_STORE_THM))
       val v = th |> concl |> rand |> rator |> rand
       val e = th |> concl |> rand |> rand
       val v_name = find_const_name (fname ^ "_v")
@@ -1108,278 +1004,10 @@ fun m_translate def = let
     val _ = print_type (type_of tm)
     val _ = print "\n\n"
     in raise UnableToTranslate tm end
-  (* DEBUG *)
     | HOL_ERR err => let
     val _ = print "\n\nml_translate: unexpected error when translating term:\n\n"
     val _ = print_thm def
     val _ = print "\n\n"
     in raise (HOL_ERR err) end;
 
-(* --- perform translation --- *)
-
-val res = translate FST;
-val res = translate SND;
-val res = translate listTheory.LENGTH;
-val res = translate listTheory.MAP;
-val res = translate MEMBER_def;
-val res = translate listTheory.EVERY_DEF;
-val res = translate listTheory.EXISTS_DEF;
-val res = translate listTheory.FILTER;
-val res = translate listTheory.APPEND;
-(* TODO: want builtin support for these *)
-val res = translate mlstringTheory.explode_aux_def;
-val res = translate mlstringTheory.explode_def;
-val explode_aux_side_thm = Q.prove(
-  `∀s n m. n + m = strlen s ==> explode_aux_side s n m `,
-  Induct_on`m` \\ rw[Once (theorem"explode_aux_side_def")]);
-val explode_side_thm = Q.prove(
-  `explode_side x`,
-  rw[definition"explode_side_def",explode_aux_side_thm])
-  |> update_precondition
-val res = translate mlstringTheory.strcat_def;
-val res = translate stringTheory.string_lt_def
-val res = translate stringTheory.string_le_def
-val res = Q.prove(`mlstring_lt x1 x2 = string_lt (explode x1) (explode x2)`,
-                simp [inv_image_def, mlstringTheory.mlstring_lt_inv_image])
-          |> translate
-val res = translate totoTheory.TO_of_LinearOrder
-val res = translate mlstringTheory.compare_aux_def
-val res = translate mlstringTheory.compare_def
-
-(* Copy and paste from mlstringProg *)
-val compare_aux_side_def = theorem"compare_aux_side_def";
-val compare_side_def = definition"compare_side_def";
-
-val compare_aux_side_thm = Q.prove (
-  `!s1 s2 ord n len. (n + len =
-    if strlen s1 < strlen s2
-      then strlen s1
-    else strlen s2) ==> compare_aux_side s1 s2 ord n len`,
-  Induct_on `len` \\ rw [Once compare_aux_side_def]
-);
-
-val compare_side_thm = Q.prove (
-  `!s1 s2. compare_side s1 s2`,
-  rw [compare_side_def, compare_aux_side_thm] ) |> update_precondition
-(* end copy and paste *)
-
-val res = translate comparisonTheory.pair_cmp_def
-val res = translate comparisonTheory.list_cmp_def
-(* -- *)
-val res = translate (subset_def |> REWRITE_RULE [MEMBER_INTRO]);
-val res = translate (holSyntaxExtraTheory.subtract_def |> REWRITE_RULE [MEMBER_INTRO]);
-val res = translate (holSyntaxExtraTheory.insert_def |> REWRITE_RULE [MEMBER_INTRO]);
-val res = translate holSyntaxExtraTheory.itlist_def;
-val res = translate holSyntaxExtraTheory.union_def;
-val res = translate mk_vartype_def;
-val res = translate is_type_def;
-val res = translate is_vartype_def;
-val res = translate holKernelPmatchTheory.rev_assocd_def;
-val res = translate holKernelTheory.type_subst_def;
-val res = translate alphavars_def;
-val res = translate holKernelPmatchTheory.raconv_def;
-val res = translate aconv_def;
-val res = translate holKernelPmatchTheory.is_var_def;
-val res = translate holKernelPmatchTheory.is_const_def;
-val res = translate holKernelPmatchTheory.is_abs_def;
-val res = translate holKernelPmatchTheory.is_comb_def;
-val res = translate mk_var_def;
-val res = translate holSyntaxExtraTheory.frees_def;
-val res = translate combinTheory.o_DEF;
-val res = translate freesl_def;
-val res = translate (freesin_def |> REWRITE_RULE [MEMBER_INTRO]);
-val res = translate holKernelPmatchTheory.vfree_in_def;
-val res = translate tyvars_def;
-val res = translate type_vars_in_term_def;
-val res = translate holSyntaxExtraTheory.variant_def;
-val res = translate vsubst_aux_def;
-val res = translate holKernelPmatchTheory.is_eq_def;
-val res = translate dest_thm_def;
-val res = translate hyp_def;
-val res = translate concl_def;
-val res = translate sortingTheory.PART_DEF;
-val res = translate sortingTheory.PARTITION_DEF;
-val res = translate sortingTheory.QSORT_DEF;
-
-val type_compare_def = tDefine "type_compare" `
-  (type_compare t1 t2 =
-     case (t1,t2) of
-     | (Tyvar x1,Tyvar x2) => mlstring$compare x1 x2
-     | (Tyvar x1,Tyapp _ _) => Less
-     | (Tyapp x1 a1,Tyvar _) => Greater
-     | (Tyapp x1 a1,Tyapp x2 a2) =>
-         case mlstring$compare x1 x2 of
-         | Equal => type_list_compare a1 a2
-         | other => other) /\
-  (type_list_compare ts1 ts2 =
-     case (ts1,ts2) of
-     | ([],[]) => Equal
-     | ([],t2::ts2) => Less
-     | (t1::ts1,[]) => Greater
-     | (t1::ts1,t2::ts2) =>
-         (case type_compare t1 t2 of
-          | Equal => type_list_compare ts1 ts2
-          | other => other))`
-  (WF_REL_TAC `measure (\x. case x of
-                  INR (x,_) => type1_size x
-                | INL (x,_) => type_size x)`)
-
-val type_cmp_thm = Q.prove(
-  `(type_cmp = type_compare) /\
-    (list_cmp type_cmp = type_list_compare)`,
-  fs [FUN_EQ_THM]
-  \\ HO_MATCH_MP_TAC (fetch "-" "type_compare_ind")
-  \\ REPEAT STRIP_TAC \\ fs []
-  \\ ONCE_REWRITE_TAC [holSyntaxExtraTheory.type_cmp_thm]
-  \\ ONCE_REWRITE_TAC [type_compare_def]
-  \\ REPEAT BasicProvers.CASE_TAC
-  \\ fs [comparisonTheory.pair_cmp_def,comparisonTheory.list_cmp_def])
-  |> CONJUNCT1;
-
-val _ = add_preferred_thy "-";
-val _ = save_thm("type_cmp_ind",
-          (fetch "-" "type_compare_ind") |> RW [GSYM type_cmp_thm]);
-val res = translate (type_compare_def |> RW [GSYM type_cmp_thm]);
-
-val term_compare_def = Define `
-  term_compare t1 t2 =
-     case (t1,t2) of
-       (Var x1 ty1,Var x2 ty2) =>
-         (case mlstring$compare x1 x2 of
-            Less => Less
-          | Equal => type_cmp ty1 ty2
-          | Greater => Greater)
-     | (Var x1 ty1,Const v52 v53) => Less
-     | (Var x1 ty1,Comb v54 v55) => Less
-     | (Var x1 ty1,Abs v56 v57) => Less
-     | (Const x1' ty1',Var v66 v67) => Greater
-     | (Const x1' ty1',Const x2' ty2') =>
-         (case mlstring$compare x1' x2' of
-            Less => Less
-          | Equal => type_cmp ty1' ty2'
-          | Greater => Greater)
-     | (Const x1' ty1',Comb v70 v71) => Less
-     | (Const x1' ty1',Abs v72 v73) => Less
-     | (Comb s1 t1,Var v82 v83) => Greater
-     | (Comb s1 t1,Const v84 v85) => Greater
-     | (Comb s1 t1,Comb s2 t2) =>
-         (case term_compare s1 s2 of
-            Less => Less
-          | Equal => term_compare t1 t2
-          | Greater => Greater)
-     | (Comb s1 t1,Abs v88 v89) => Less
-     | (Abs s1' t1',Var v98 v99) => Greater
-     | (Abs s1' t1',Const v100 v101) => Greater
-     | (Abs s1' t1',Comb v102 v103) => Greater
-     | (Abs s1' t1',Abs s2' t2') =>
-         case term_compare s1' s2' of
-           Less => Less
-         | Equal => term_compare t1' t2'
-         | Greater => Greater`;
-
-val term_cmp_thm = Q.prove(
-  `term_cmp = term_compare`,
-  fs [FUN_EQ_THM]
-  \\ HO_MATCH_MP_TAC (fetch "-" "term_compare_ind")
-  \\ REPEAT STRIP_TAC \\ fs []
-  \\ ONCE_REWRITE_TAC [holSyntaxExtraTheory.term_cmp_thm]
-  \\ ONCE_REWRITE_TAC [term_compare_def]
-  \\ REPEAT BasicProvers.CASE_TAC
-  \\ fs [comparisonTheory.pair_cmp_def])
-
-val _ = add_preferred_thy "-";
-val _ = save_thm("term_cmp_ind",
-          (fetch "-" "term_compare_ind") |> RW [GSYM term_cmp_thm]);
-val res = translate (term_compare_def |> RW [GSYM term_cmp_thm]);
-
-val res = translate holKernelPmatchTheory.codomain_def;
-val res = translate holSyntaxTheory.typeof_def;
-val res = translate holSyntaxTheory.ordav_def;
-val res = translate holSyntaxTheory.orda_def;
-val res = translate holSyntaxTheory.term_remove_def;
-val res = translate holSyntaxTheory.term_union_def;
-
-(* DEBUG *)
-val def = vsubst_def;
-m_translate def;
-val tm = (def (* rec *) |> m_translate; ``T``) handle BREAKPOINT tm => tm;
-(* END DEBUG *)
-
-val def = assoc_def   (* rec *) |> m_translate
-val def = map_def    (* rec *) |> m_translate
-val def = forall_def (* rec *) |> m_translate
-val def = dest_type_def |> m_translate
-val def = dest_vartype_def |> m_translate
-val def = holKernelPmatchTheory.dest_var_def |> m_translate
-val def = holKernelPmatchTheory.dest_const_def |> m_translate
-val def = holKernelPmatchTheory.dest_comb_def |> m_translate
-val def = holKernelPmatchTheory.dest_abs_def |> m_translate
-val def = holKernelPmatchTheory.rator_def |> m_translate
-val def = holKernelPmatchTheory.rand_def |> m_translate
-val def = holKernelPmatchTheory.dest_eq_def |> m_translate
-val def = holKernelPmatchTheory.mk_abs_def |> m_translate
-val def = get_type_arity_def |> m_translate
-val def = mk_type_def |> m_translate
-val def = mk_fun_ty_def |> m_translate
-val def = holKernelPmatchTheory.type_of_def |> m_translate
-val def = get_const_type_def |> m_translate
-val def = holKernelPmatchTheory.mk_comb_def |> m_translate
-val def = can_def |> m_translate
-val def = mk_const_def |> m_translate
-val def = image_def |> m_translate
-
-val fdM_def = new_definition("fdM_def",``fdM = first_dup``)
-val fdM_intro = SYM fdM_def
-val fdM_ind = save_thm("fdM_ind",REWRITE_RULE[MEMBER_INTRO]first_dup_ind)
-val fdM_eqs = REWRITE_RULE[MEMBER_INTRO,fdM_intro]first_dup_def
-val def = fdM_eqs |> translate
-val def = REWRITE_RULE[fdM_intro]add_constants_def |> m_translate
-val def = add_def_def |> m_translate
-val def = new_constant_def |> m_translate
-val def = add_type_def |> m_translate
-val def = new_type_def |> m_translate
-val def = holKernelPmatchTheory.EQ_MP_def |> m_translate
-val def = ASSUME_def |> m_translate
-val def = new_axiom_def |> m_translate
-val def = vsubst_def |> m_translate
-val def = inst_aux_def (* rec *) |> m_translate
-val def = inst_def |> m_translate
-val def = mk_eq_def |> m_translate
-val def = REFL_def |> m_translate
-val def = holKernelPmatchTheory.TRANS_def |> m_translate
-val def = holKernelPmatchTheory.MK_COMB_def |> m_translate
-val def = holKernelPmatchTheory.ABS_def |> m_translate
-val def = holKernelPmatchTheory.BETA_def |> m_translate
-val def = DEDUCT_ANTISYM_RULE_def |> m_translate
-val def = new_specification_def |> m_translate
-val def = new_basic_definition_def |> m_translate
-val def = (INST_TYPE_def |> SIMP_RULE std_ss [LET_DEF]) |> m_translate
-val def = (INST_def |> SIMP_RULE std_ss [LET_DEF]) |> m_translate
-val def = new_basic_type_definition_def |> m_translate
-val def = holKernelPmatchTheory.SYM_def |> m_translate
-val def = PROVE_HYP_def |> m_translate
-val def = list_to_hypset_def |> translate
-val def = ALPHA_THM_def |> m_translate
-
-val _ = ml_prog_update (close_module NONE); (* TODO: needs signature SOME ... *)
-
-(* extract the interesting thm *)
-
-val _ = Globals.max_print_depth := 10;
-
-fun define_abbrev_conv name tm = let
-  val def = define_abbrev true name tm
-  in GSYM def |> SPEC_ALL end
-
-val candle_prog_thm =
-  get_thm (get_curr_prog_state ())
-  |> REWRITE_RULE [ML_code_def]
-  |> CONV_RULE ((RATOR_CONV o RATOR_CONV o RAND_CONV)
-                (EVAL THENC define_abbrev_conv "candle_code"))
-  |> CONV_RULE ((RATOR_CONV o RAND_CONV)
-                (EVAL THENC define_abbrev_conv "candle_init_env"))
-  |> CONV_RULE ((RAND_CONV)
-                (EVAL THENC define_abbrev_conv "candle_init_state"))
-  |> curry save_thm "candle_prog_thm"
-
-val _ = export_theory();
+end
